swapped names of invs_dv_next_2 and invs_dv_next_3

src/proofs/no_slashable_attestations/supporting_lemmas/dv_next_preserves_ind_inv/invs_dv_next_2.dfy
@@ -3,17 +3,16 @@ include "../../common/attestation_creation_instrumented.dfy"
 include "../../../../specs/consensus/consensus.dfy"
 include "../../../../specs/network/network.dfy"
 include "../../../../specs/dv/dv_attestation_creation.dfy"
+include "../../../../specs/dvc/dvc_attestation_creation.dfy"
 
 include "../../../common/helper_sets_lemmas.dfy"
-include "../../common/common_proofs.dfy"
-include "../../common/dvc_spec_axioms.dfy"
+include "../../../no_slashable_attestations/common/common_proofs.dfy"
+include "../../../no_slashable_attestations/common/dvc_spec_axioms.dfy"
 
-include "../inv.dfy"
-
-include "invs_fnc_1.dfy"
-include "invs_fnc_2.dfy"
 include "invs_dv_next_1.dfy"
-include "invs_dv_next_3.dfy"
+include "../inv.dfy"
+include "../../../common/helper_pred_fcn.dfy"
+
 
 module Invs_DV_Next_2
 {
@@ -22,690 +21,2219 @@ module Invs_DV_Next_2
     import opened ConsensusSpec
     import opened NetworkSpec
     import opened DVC_Spec
-    import opened DV
+    import opened DV    
     import opened Att_Inv_With_Empty_Initial_Attestation_Slashing_DB
-    import opened Fnc_Invs_1
     import opened Helper_Sets_Lemmas
+    import opened Common_Proofs
     import opened Invs_DV_Next_1
-    import opened Fnc_Invs_2
+    import DVC_Spec_NonInstr
     import opened DVC_Spec_Axioms
-    import opened Invs_DV_Next_3
+    import opened Helper_Pred_Fcn
 
-    lemma lem_inv_att_slashing_db_hist_keeps_track_of_only_rcvd_att_duties_dv_next(
-        dv: DVState,
-        event: DV.Event,
-        dv': DVState
-    )    
-    requires NextEventPreCond(dv, event)
-    requires NextEvent(dv, event, dv')    
-    requires inv_consensus_instance_only_for_slot_in_which_dvc_has_rcvd_att_duty(dv)
-    requires inv_att_slashing_db_hist_keeps_track_of_only_rcvd_att_duties(dv)  
-    ensures inv_att_slashing_db_hist_keeps_track_of_only_rcvd_att_duties(dv')
-    {        
-        match event 
-        {
-            case HonestNodeTakingStep(node, nodeEvent, nodeOutputs) =>
-                var dvc := dv.honest_nodes_states[node];
-                var dvc' := dv'.honest_nodes_states[node];                
-                
-                match nodeEvent
-                {
-                    case ServeAttstationDuty(attestation_duty) =>   
-                        assert inv_consensus_instance_only_for_slot_in_which_dvc_has_rcvd_att_duty_body(dvc);   
-                        assert inv_att_slashing_db_hist_keeps_track_of_only_rcvd_att_duties_body(dvc);                                           
-                        lem_inv_att_slashing_db_hist_keeps_track_of_only_rcvd_att_duties_body_f_serve_attestation_duty(dvc, attestation_duty, dvc');
-                        assert inv_att_slashing_db_hist_keeps_track_of_only_rcvd_att_duties_body(dvc');
-                        
-                    case AttConsensusDecided(id, decided_attestation_data) => 
-                        lem_inv_att_slashing_db_hist_keeps_track_of_only_rcvd_att_duties_body_f_att_consensus_decided(dvc, id, decided_attestation_data, dvc');
-                        assert inv_att_slashing_db_hist_keeps_track_of_only_rcvd_att_duties_body(dvc');
-                        
-                    case ReceivedAttestationShare(attestation_share) =>                         
-                        lem_inv_att_slashing_db_hist_keeps_track_of_only_rcvd_att_duties_body_f_listen_for_attestation_shares(dvc, attestation_share, dvc');
-                        assert inv_att_slashing_db_hist_keeps_track_of_only_rcvd_att_duties_body(dvc');
-                       
-                    case ImportedNewBlock(block) => 
-                        var dvc_mod := f_add_block_to_bn(dvc, block);
-                        lem_inv_att_slashing_db_hist_keeps_track_of_only_rcvd_att_duties_body_f_add_block_to_bn(dvc, block, dvc_mod);
-                        assert inv_att_slashing_db_hist_keeps_track_of_only_rcvd_att_duties_body(dvc_mod);
-                        lem_inv_att_slashing_db_hist_keeps_track_of_only_rcvd_att_duties_body_f_listen_for_new_imported_blocks(dvc_mod, block, dvc');                        
-                        assert inv_att_slashing_db_hist_keeps_track_of_only_rcvd_att_duties_body(dvc');
-
-                    case ResendAttestationShares =>                                                                      
-
-                    case NoEvent => 
-                        
-                }
-                
-            case AdeversaryTakingStep(node, new_attestation_share_sent, messagesReceivedByTheNode) =>
-                
-        }   
-    }
-
-    lemma lem_inv_exists_db_in_att_slashing_db_hist_for_every_validity_pred_dv_next(
-        dv: DVState,
-        event: DV.Event,
-        dv': DVState
-    )    
-    requires NextEventPreCond(dv, event)
-    requires NextEvent(dv, event, dv')    
-    requires inv_consensus_instances_only_for_rcvd_duties(dv)
-    requires inv_exists_db_in_att_slashing_db_hist_for_every_validity_pred(dv)  
-    // ensures inv_exists_db_in_att_slashing_db_hist_for_every_validity_pred(dv')
-    {        
-        match event 
-        {
-            case HonestNodeTakingStep(node, nodeEvent, nodeOutputs) =>
-                var dvc := dv.honest_nodes_states[node];
-                var dvc' := dv'.honest_nodes_states[node];                
-                
-                match nodeEvent
-                {
-                    case ServeAttstationDuty(attestation_duty) =>   
-                        
-                        assert inv_consensus_instances_only_for_rcvd_duties_body(dvc);   
-                        assert inv_exists_db_in_att_slashing_db_hist_for_every_validity_pred_body(dvc);                                           
-                        lem_inv_exists_db_in_att_slashing_db_hist_for_every_validity_pred_body_f_serve_attestation_duty(dvc, attestation_duty, dvc');
-                        assert inv_exists_db_in_att_slashing_db_hist_for_every_validity_pred_body(dvc');
-                        
-                    case AttConsensusDecided(id, decided_attestation_data) => 
-                        lem_inv_exists_db_in_att_slashing_db_hist_for_every_validity_pred_body_f_att_consensus_decided(dvc, id, decided_attestation_data, dvc');
-                        assert inv_exists_db_in_att_slashing_db_hist_for_every_validity_pred_body(dvc');
-                        
-                    case ReceivedAttestationShare(attestation_share) =>                         
-                        lem_inv_exists_db_in_att_slashing_db_hist_for_every_validity_pred_body_f_listen_for_attestation_shares(dvc, attestation_share, dvc');
-                        assert inv_exists_db_in_att_slashing_db_hist_for_every_validity_pred_body(dvc');
-                       
-                    case ImportedNewBlock(block) => 
-                        var dvc_mod := f_add_block_to_bn(dvc, block);
-                        lem_inv_exists_db_in_att_slashing_db_hist_for_every_validity_pred_body_f_add_block_to_bn(dvc, block, dvc_mod);
-                        assert inv_exists_db_in_att_slashing_db_hist_for_every_validity_pred_body(dvc_mod);
-                        lem_inv_exists_db_in_att_slashing_db_hist_for_every_validity_pred_body_f_listen_for_new_imported_blocks(dvc_mod, block, dvc');                        
-                        assert inv_exists_db_in_att_slashing_db_hist_for_every_validity_pred_body(dvc');
-
-                    case ResendAttestationShares =>                                                                      
-
-                    case NoEvent => 
-                        
-                }
-                
-            case AdeversaryTakingStep(node, new_attestation_share_sent, messagesReceivedByTheNode) =>
-                
-        }   
-    }
-
-    lemma lem_inv_validity_pred_for_slot_k_is_stored_in_att_slashing_db_hist_k_dv_next(
-        dv: DVState,
-        event: DV.Event,
-        dv': DVState
-    )    
-    requires NextEventPreCond(dv, event)
-    requires NextEvent(dv, event, dv')    
-    requires inv_consensus_instance_only_for_slot_in_which_dvc_has_rcvd_att_duty(dv)
-    requires inv_validity_pred_for_slot_k_is_stored_in_att_slashing_db_hist_k(dv)  
-    ensures inv_validity_pred_for_slot_k_is_stored_in_att_slashing_db_hist_k(dv')
-    {        
-        match event 
-        {
-            case HonestNodeTakingStep(node, nodeEvent, nodeOutputs) =>
-                var dvc := dv.honest_nodes_states[node];
-                var dvc' := dv'.honest_nodes_states[node];                
-                
-                match nodeEvent
-                {
-                    case ServeAttstationDuty(attestation_duty) =>   
-                        
-                        assert inv_consensus_instance_only_for_slot_in_which_dvc_has_rcvd_att_duty_body(dvc);   
-                        assert inv_validity_pred_for_slot_k_is_stored_in_att_slashing_db_hist_k_body(dvc);                                           
-                        lem_inv_validity_pred_for_slot_k_is_stored_in_att_slashing_db_hist_k_body_f_serve_attestation_duty(dvc, attestation_duty, dvc');
-                        assert inv_validity_pred_for_slot_k_is_stored_in_att_slashing_db_hist_k_body(dvc');
-                        
-                    case AttConsensusDecided(id, decided_attestation_data) => 
-                        lem_inv_validity_pred_for_slot_k_is_stored_in_att_slashing_db_hist_k_body_f_att_consensus_decided(dvc, id, decided_attestation_data, dvc');
-                        assert inv_validity_pred_for_slot_k_is_stored_in_att_slashing_db_hist_k_body(dvc');
-                        
-                    case ReceivedAttestationShare(attestation_share) =>                         
-                        lem_inv_validity_pred_for_slot_k_is_stored_in_att_slashing_db_hist_k_body_f_listen_for_attestation_shares(dvc, attestation_share, dvc');
-                        assert inv_validity_pred_for_slot_k_is_stored_in_att_slashing_db_hist_k_body(dvc');
-                       
-                    case ImportedNewBlock(block) => 
-                        var dvc_mod := f_add_block_to_bn(dvc, block);
-                        lem_inv_validity_pred_for_slot_k_is_stored_in_att_slashing_db_hist_k_body_f_add_block_to_bn(dvc, block, dvc_mod);
-                        assert inv_validity_pred_for_slot_k_is_stored_in_att_slashing_db_hist_k_body(dvc_mod);
-                        lem_inv_validity_pred_for_slot_k_is_stored_in_att_slashing_db_hist_k_body_f_listen_for_new_imported_blocks(dvc_mod, block, dvc');                        
-                        assert inv_validity_pred_for_slot_k_is_stored_in_att_slashing_db_hist_k_body(dvc');
-
-                    case ResendAttestationShares =>                                                                      
-
-                    case NoEvent => 
-                        
-                }
-                
-            case AdeversaryTakingStep(node, new_attestation_share_sent, messagesReceivedByTheNode) =>
-                
-        }   
-    }
-
-    lemma lem_inv_monotonic_att_slashing_db_dv_next(
-        dv: DVState,
-        event: DV.Event,
-        dv': DVState
-    )    
-    requires NextEventPreCond(dv, event)
-    requires NextEvent(dv, event, dv')    
-    ensures inv_monotonic_att_slashing_db(dv, event, dv')
-    {        
-        match event 
-        {
-            case HonestNodeTakingStep(node, nodeEvent, nodeOutputs) =>
-                var dvc := dv.honest_nodes_states[node];
-                var dvc' := dv'.honest_nodes_states[node];                
-                
-                match nodeEvent
-                {
-                    case ServeAttstationDuty(attestation_duty) =>   
-                        lem_inv_monotonic_att_slashing_db_body_f_serve_attestation_duty(dvc, attestation_duty, dvc');
-                        assert inv_monotonic_att_slashing_db_body(dvc, dvc');
-                        
-                    case AttConsensusDecided(id, decided_attestation_data) => 
-                        lem_inv_monotonic_att_slashing_db_body_f_att_consensus_decided(dvc, id, decided_attestation_data, dvc');
-                        assert inv_monotonic_att_slashing_db_body(dvc, dvc');
-                        
-                    case ReceivedAttestationShare(attestation_share) =>                         
-                        lem_inv_monotonic_att_slashing_db_body_f_listen_for_attestation_shares(dvc, attestation_share, dvc');
-                        assert inv_monotonic_att_slashing_db_body(dvc, dvc');
-                       
-                    case ImportedNewBlock(block) => 
-                        var dvc_mod := f_add_block_to_bn(dvc, block);
-                        lem_inv_monotonic_att_slashing_db_body_f_add_block_to_bn(dvc, block, dvc_mod);
-                        assert inv_monotonic_att_slashing_db_body(dvc, dvc_mod);
-                        lem_inv_monotonic_att_slashing_db_body_f_listen_for_new_imported_blocks(dvc_mod, block, dvc');                        
-                        assert inv_monotonic_att_slashing_db_body(dvc_mod, dvc');
-
-                    case ResendAttestationShares =>                                                                      
-
-                    case NoEvent => 
-                        
-                }
-                
-            case AdeversaryTakingStep(node, new_attestation_share_sent, messagesReceivedByTheNode) =>
-                
-        }   
-    }
-
-    lemma lem_inv_every_db_in_att_slashing_db_hist_is_subset_of_att_slashing_db_dv_next(
-        dv: DVState,
-        event: DV.Event,
-        dv': DVState
-    )    
-    requires NextEventPreCond(dv, event)
-    requires NextEvent(dv, event, dv')    
-    requires inv_consensus_instances_only_for_rcvd_duties(dv)
-    requires inv_every_db_in_att_slashing_db_hist_is_subset_of_att_slashing_db(dv)  
-    ensures inv_every_db_in_att_slashing_db_hist_is_subset_of_att_slashing_db(dv')
-    {        
-        match event 
-        {
-            case HonestNodeTakingStep(node, nodeEvent, nodeOutputs) =>
-                var dvc := dv.honest_nodes_states[node];
-                var dvc' := dv'.honest_nodes_states[node];                
-                
-                match nodeEvent
-                {
-                    case ServeAttstationDuty(attestation_duty) =>   
-                        
-                        assert inv_consensus_instances_only_for_rcvd_duties_body(dvc);   
-                        assert inv_every_db_in_att_slashing_db_hist_is_subset_of_att_slashing_db_body(dvc);                                           
-                        lem_inv_every_db_in_att_slashing_db_hist_is_subset_of_att_slashing_db_body_f_serve_attestation_duty(dvc, attestation_duty, dvc');
-                        assert inv_every_db_in_att_slashing_db_hist_is_subset_of_att_slashing_db_body(dvc');
-                        
-                    case AttConsensusDecided(id, decided_attestation_data) => 
-                        lem_inv_every_db_in_att_slashing_db_hist_is_subset_of_att_slashing_db_body_f_att_consensus_decided(dvc, id, decided_attestation_data, dvc');
-                        assert inv_every_db_in_att_slashing_db_hist_is_subset_of_att_slashing_db_body(dvc');
-                        
-                    case ReceivedAttestationShare(attestation_share) =>                         
-                        lem_inv_every_db_in_att_slashing_db_hist_is_subset_of_att_slashing_db_body_f_listen_for_attestation_shares(dvc, attestation_share, dvc');
-                        assert inv_every_db_in_att_slashing_db_hist_is_subset_of_att_slashing_db_body(dvc');
-                       
-                    case ImportedNewBlock(block) => 
-                        var dvc_mod := f_add_block_to_bn(dvc, block);
-                        lem_inv_every_db_in_att_slashing_db_hist_is_subset_of_att_slashing_db_body_f_add_block_to_bn(dvc, block, dvc_mod);
-                        assert inv_every_db_in_att_slashing_db_hist_is_subset_of_att_slashing_db_body(dvc_mod);
-                        lem_inv_every_db_in_att_slashing_db_hist_is_subset_of_att_slashing_db_body_f_listen_for_new_imported_blocks(dvc_mod, block, dvc');                        
-                        assert inv_every_db_in_att_slashing_db_hist_is_subset_of_att_slashing_db_body(dvc');
-
-                    case ResendAttestationShares =>                                                                      
-
-                    case NoEvent => 
-                        
-                }
-                
-            case AdeversaryTakingStep(node, new_attestation_share_sent, messagesReceivedByTheNode) =>
-                
-        }   
-    }
-
-    lemma lem_inv_monotonic_att_slashing_db_hist_dv_next(
-        dv: DVState,
-        event: DV.Event,
-        dv': DVState
-    )    
-    requires NextEventPreCond(dv, event)
-    requires NextEvent(dv, event, dv')    
-    ensures inv_monotonic_att_slashing_db_hist(dv, event, dv')
-    {        
-        match event 
-        {
-            case HonestNodeTakingStep(node, nodeEvent, nodeOutputs) =>
-                var dvc := dv.honest_nodes_states[node];
-                var dvc' := dv'.honest_nodes_states[node];                
-                
-                match nodeEvent
-                {
-                    case ServeAttstationDuty(attestation_duty) =>   
-                        lem_inv_monotonic_att_slashing_db_hist_body_f_serve_attestation_duty(dvc, attestation_duty, dvc');
-                        assert inv_monotonic_att_slashing_db_hist_body(dvc, dvc');
-                        
-                    case AttConsensusDecided(id, decided_attestation_data) => 
-                        lem_inv_monotonic_att_slashing_db_hist_body_f_att_consensus_decided(dvc, id, decided_attestation_data, dvc');
-                        assert inv_monotonic_att_slashing_db_hist_body(dvc, dvc');
-                        
-                    case ReceivedAttestationShare(attestation_share) =>                         
-                        lem_inv_monotonic_att_slashing_db_hist_body_f_listen_for_attestation_shares(dvc, attestation_share, dvc');
-                        assert inv_monotonic_att_slashing_db_hist_body(dvc, dvc');
-                       
-                    case ImportedNewBlock(block) => 
-                        var dvc_mod := f_add_block_to_bn(dvc, block);
-                        lem_inv_monotonic_att_slashing_db_hist_body_f_add_block_to_bn(dvc, block, dvc_mod);
-                        assert inv_monotonic_att_slashing_db_hist_body(dvc, dvc_mod);
-                        lem_inv_monotonic_att_slashing_db_hist_body_f_listen_for_new_imported_blocks(dvc_mod, block, dvc');                        
-                        assert inv_monotonic_att_slashing_db_hist_body(dvc_mod, dvc');
-
-                    case ResendAttestationShares =>                                                                      
-
-                    case NoEvent => 
-                        
-                }
-                
-            case AdeversaryTakingStep(node, new_attestation_share_sent, messagesReceivedByTheNode) =>
-                
-        }   
-    }
-
-    lemma lem_inv_active_attn_consensus_instances_are_tracked_in_att_slashing_db_hist_dv_next(
-        dv: DVState,
-        event: DV.Event,
-        dv': DVState
-    )    
-    requires NextEventPreCond(dv, event)
-    requires NextEvent(dv, event, dv')    
-    requires inv_active_attn_consensus_instances_are_tracked_in_att_slashing_db_hist(dv)
-    ensures inv_active_attn_consensus_instances_are_tracked_in_att_slashing_db_hist(dv')
-    {        
-        match event 
-        {
-            case HonestNodeTakingStep(node, nodeEvent, nodeOutputs) =>
-                var dvc := dv.honest_nodes_states[node];
-                var dvc' := dv'.honest_nodes_states[node];                
-                
-                match nodeEvent
-                {
-                    case ServeAttstationDuty(attestation_duty) =>   
-                        lem_inv_active_attn_consensus_instances_are_tracked_in_att_slashing_db_hist_body_f_serve_attestation_duty(dvc, attestation_duty, dvc');
-                        assert inv_active_attn_consensus_instances_are_tracked_in_att_slashing_db_hist_body(dvc');
-                        
-                    case AttConsensusDecided(id, decided_attestation_data) => 
-                        lem_inv_active_attn_consensus_instances_are_tracked_in_att_slashing_db_hist_body_f_att_consensus_decided(dvc, id, decided_attestation_data, dvc');
-                        assert inv_active_attn_consensus_instances_are_tracked_in_att_slashing_db_hist_body(dvc');
-                        
-                    case ReceivedAttestationShare(attestation_share) =>                         
-                        lem_inv_active_attn_consensus_instances_are_tracked_in_att_slashing_db_hist_body_f_listen_for_attestation_shares(dvc, attestation_share, dvc');
-                        assert inv_active_attn_consensus_instances_are_tracked_in_att_slashing_db_hist_body(dvc');
-                       
-                    case ImportedNewBlock(block) => 
-                        var dvc_mod := f_add_block_to_bn(dvc, block);
-                        lem_inv_active_attn_consensus_instances_are_tracked_in_att_slashing_db_hist_body_f_add_block_to_bn(dvc, block, dvc_mod);
-                        assert inv_active_attn_consensus_instances_are_tracked_in_att_slashing_db_hist_body(dvc_mod);
-                        lem_inv_active_attn_consensus_instances_are_tracked_in_att_slashing_db_hist_body_f_listen_for_new_imported_blocks(dvc_mod, block, dvc');                        
-                        assert inv_active_attn_consensus_instances_are_tracked_in_att_slashing_db_hist_body(dvc');
-
-                    case ResendAttestationShares =>                                                                      
-
-                    case NoEvent => 
-                        
-                }
-                
-            case AdeversaryTakingStep(node, new_attestation_share_sent, messagesReceivedByTheNode) =>
-                
-        }   
-    }
-
-    lemma lem_inv_construct_signed_attestation_signature_assumptions_helper_dv_next(
-        dv: DVState,
-        event: DV.Event,
-        dv': DVState
-    )    
-    requires NextEventPreCond(dv, event)
-    requires NextEvent(dv, event, dv')    
-    requires inv_construct_signed_attestation_signature_assumptions_helper(dv)
-    ensures inv_construct_signed_attestation_signature_assumptions_helper(dv')    
-    {
-        assert dv.construct_signed_attestation_signature == dv'.construct_signed_attestation_signature;
-    }
-
-    lemma lem_inv_all_in_transit_messages_were_sent_body_network_spec_next<M>(
-        e: Network<M>,
-        e': Network<M>,
-        n: BLSPubkey,
-        messagesToBeSent: set<MessaageWithRecipient<M>>,
-        messagesReceived: set<M>
+    predicate pred_the_latest_attestation_duty_was_sent_from_dv(
+        s': DVState,
+        index_next_attestation_duty_to_be_served: nat,
+        attestation_duty: AttestationDuty,
+        node: BLSPubkey
     )
-    requires NetworkSpec.Next(e, e', n, messagesToBeSent, messagesReceived)
-    requires inv_all_in_transit_messages_were_sent_body(e)
-    ensures inv_all_in_transit_messages_were_sent_body(e')
-    {}
+    {
+        && index_next_attestation_duty_to_be_served > 0
+        && var an := s'.sequence_attestation_duties_to_be_served[index_next_attestation_duty_to_be_served - 1];
+        && attestation_duty == an.attestation_duty
+        && node == an.node    
+    }    
+
+    lemma lem_ServeAttstationDuty2_helper(
+        s: DVState,
+        node: BLSPubkey,
+        nodeEvent: Types.Event,
+        nodeOutputs: DVC_Spec.Outputs,
+        s': DVState
+    )
+    requires NextHonestAfterAddingBlockToBn.requires(s, node, nodeEvent, nodeOutputs, s' );
+    requires NextHonestAfterAddingBlockToBn(s, node, nodeEvent, nodeOutputs, s' );  
+    requires nodeEvent.ServeAttstationDuty?
+    ensures s'.index_next_attestation_duty_to_be_served > 0
+    ensures && pred_the_latest_attestation_duty_was_sent_from_dv(s', s'.index_next_attestation_duty_to_be_served, nodeEvent.attestation_duty, node )
+            && s.index_next_attestation_duty_to_be_served == s'.index_next_attestation_duty_to_be_served - 1;
+    {
+
+        var s_node := s.honest_nodes_states[node];
+        var s'_node := s'.honest_nodes_states[node];
+        assert  NextHonestAfterAddingBlockToBn.requires(add_block_to_bn_with_event(s, node, nodeEvent), node, nodeEvent, nodeOutputs, s' );
+        assert  NextHonestAfterAddingBlockToBn(add_block_to_bn_with_event(s, node, nodeEvent), node, nodeEvent, nodeOutputs, s' );
+
+        match nodeEvent
+        {
+            case ServeAttstationDuty(attestation_duty) => 
+                assert s.sequence_attestation_duties_to_be_served == s'.sequence_attestation_duties_to_be_served;
+                assert s.index_next_attestation_duty_to_be_served == s'.index_next_attestation_duty_to_be_served - 1;
+
+                var an := s'.sequence_attestation_duties_to_be_served[s'.index_next_attestation_duty_to_be_served - 1];
+
+                assert attestation_duty == an.attestation_duty;
+                assert node == an.node;
+        }
+    }     
+
+    // // TODO: Rename to lem_ServeAttstationDuty
+    lemma lem_ServeAttstationDuty(
+        s: DVState,
+        event: DV.Event,
+        s': DVState
+    )
+    requires NextEventPreCond(s, event)
+    requires NextEvent(s, event, s')    
+    requires event.HonestNodeTakingStep?
+    requires event.event.ServeAttstationDuty?
+    ensures s'.index_next_attestation_duty_to_be_served > 0
+    ensures && pred_the_latest_attestation_duty_was_sent_from_dv(s', s'.index_next_attestation_duty_to_be_served, event.event.attestation_duty, event.node )
+            && s.index_next_attestation_duty_to_be_served == s'.index_next_attestation_duty_to_be_served - 1;
+    {
+        assert s.att_network.allMessagesSent <= s'.att_network.allMessagesSent;
+        match event 
+        {
+            case HonestNodeTakingStep(node, nodeEvent, nodeOutputs) =>
+                var s_node := s.honest_nodes_states[node];
+                var s'_node := s'.honest_nodes_states[node];
+                assert  NextHonestAfterAddingBlockToBn.requires(add_block_to_bn_with_event(s, node, nodeEvent), node, nodeEvent, nodeOutputs, s' );
+                assert  NextHonestAfterAddingBlockToBn(add_block_to_bn_with_event(s, node, nodeEvent), node, nodeEvent, nodeOutputs, s' );
+                lem_ServeAttstationDuty2_helper(add_block_to_bn_with_event(s, node, nodeEvent), node, nodeEvent, nodeOutputs, s' );
+        }        
+    }    
+
+    lemma lem_f_serve_attestation_duty_constants(
+        s: DVCState,
+        attestation_duty: AttestationDuty,
+        s': DVCState
+    )  
+    requires f_serve_attestation_duty.requires(s, attestation_duty)
+    requires s' == f_serve_attestation_duty(s, attestation_duty).state
+    ensures s'.bn.attestations_submitted == s.bn.attestations_submitted      
+    ensures s'.rcvd_attestation_shares == s.rcvd_attestation_shares
+    ensures f_serve_attestation_duty(s, attestation_duty).outputs == getEmptyOuputs()
+    { }
+
+    lemma lem_f_check_for_next_duty_unchanged_dvc_vars(
+        s: DVCState,
+        attestation_duty: AttestationDuty,
+        s': DVCState
+    )
+    requires f_check_for_next_duty.requires(s, attestation_duty)
+    requires s' == f_check_for_next_duty(s, attestation_duty).state
+    ensures s'.bn.attestations_submitted == s.bn.attestations_submitted
+    ensures s'.rcvd_attestation_shares == s.rcvd_attestation_shares
+    ensures f_check_for_next_duty(s, attestation_duty).outputs == getEmptyOuputs()
+    { }
+
+    lemma lem_f_att_consensus_decided_unchanged_dvc_vars(
+        s: DVCState,
+        id: Slot,
+        decided_attestation_data: AttestationData,        
+        s': DVCState
+    )
+    requires f_att_consensus_decided.requires(s, id, decided_attestation_data)
+    requires s' == f_att_consensus_decided(s, id, decided_attestation_data).state
+    ensures s'.bn.attestations_submitted == s.bn.attestations_submitted
+    ensures s'.rcvd_attestation_shares == s.rcvd_attestation_shares
+    { } 
+
+    // // Note: Lemma's name should be revisited due to second postcondition
+    lemma lem_f_listen_for_new_imported_blocksd_unchanged_dvc_vars(
+        s: DVCState,
+        block: BeaconBlock,
+        s': DVCState
+    )
+    requires f_listen_for_new_imported_blocks.requires(s, block)
+    requires s' == f_listen_for_new_imported_blocks(s, block).state
+    ensures s'.bn.attestations_submitted == s.bn.attestations_submitted
+    ensures s'.rcvd_attestation_shares.Keys <= s.rcvd_attestation_shares.Keys
+    ensures forall k | k in s'.rcvd_attestation_shares.Keys :: s'.rcvd_attestation_shares[k] == s.rcvd_attestation_shares[k]
+    ensures f_listen_for_new_imported_blocks(s, block).outputs == getEmptyOuputs()
+    { }  
+
+    lemma lem_f_listen_for_attestation_shares_unchanged_dvc_vars(
+        s: DVCState,
+        attestation_share: AttestationShare,
+        s': DVCState
+    )
+    requires f_listen_for_attestation_shares.requires(s, attestation_share)
+    requires s' == f_listen_for_attestation_shares(s, attestation_share).state    
+    ensures s'.attestation_consensus_engine_state == s.attestation_consensus_engine_state
+    ensures s'.attestation_consensus_engine_state.att_slashing_db_hist == s.attestation_consensus_engine_state.att_slashing_db_hist
+    ensures s'.latest_attestation_duty == s.latest_attestation_duty
+    ensures s'.current_attestation_duty == s.current_attestation_duty
+    ensures s'.attestation_slashing_db == s.attestation_slashing_db
+    ensures s'.future_att_consensus_instances_already_decided == s.future_att_consensus_instances_already_decided
+    { }
+
+    lemma lem_f_resend_attestation_share_unchanged_dvc_vars(
+        s: DVCState,
+        s': DVCState
+    )
+    requires f_resend_attestation_share.requires(s)
+    requires s' == f_resend_attestation_share(s).state    
+    ensures s'.attestation_consensus_engine_state == s.attestation_consensus_engine_state
+    ensures s'.attestation_consensus_engine_state.att_slashing_db_hist == s.attestation_consensus_engine_state.att_slashing_db_hist
+    ensures s'.latest_attestation_duty == s.latest_attestation_duty
+    ensures s'.current_attestation_duty == s.current_attestation_duty
+    ensures s'.attestation_slashing_db == s.attestation_slashing_db
+    ensures s'.future_att_consensus_instances_already_decided == s.future_att_consensus_instances_already_decided
+    { }    
+
+    function recover_bls_signature(
+        r: Root,
+        signature: BLSSignature
+    ): BLSPubkey
+    requires exists pubkey :: verify_bls_siganture(r, signature, pubkey)
+    {
+        var pubkey :| verify_bls_siganture(r, signature, pubkey);
+        pubkey
+    }
+
+    lemma lem_recover_bls_signature()
+    ensures forall r, s1, s2 |
+                && recover_bls_signature.requires(r, s1)
+                && recover_bls_signature.requires(r, s2)
+                && recover_bls_signature(r, s1) == recover_bls_signature(r, s2)
+            ::
+                s1 == s2
+    {
+        lem_verify_bls_siganture();
+    }
+
+    lemma lem_inv_exists_honest_dvc_that_sent_att_share_for_submitted_att_f_listen_for_attestation_shares(
+        process: DVCState,
+        attestation_share: AttestationShare,
+        s': DVCState,
+        dv: DVState
+    )
+    requires f_listen_for_attestation_shares.requires(process, attestation_share)
+    requires s' == f_listen_for_attestation_shares(process, attestation_share).state
+    requires construct_signed_attestation_signature_assumptions_helper(
+        process.construct_signed_attestation_signature,
+        process.dv_pubkey,
+        dv.all_nodes
+    )
+    requires inv_quorum_constraints(dv)
+    requires attestation_share in dv.att_network.allMessagesSent
+    requires pred_rcvd_attestation_shares_is_in_all_messages_sent_single_node_state(dv, process)
+    requires ( forall a | a in process.bn.attestations_submitted :: exists hn', att_share: AttestationShare ::
+                    inv_exists_honest_dvc_that_sent_att_share_for_submitted_att_body(dv, hn', att_share, a)
+             )
+    ensures forall a | a in s'.bn.attestations_submitted :: exists hn', att_share: AttestationShare :: inv_exists_honest_dvc_that_sent_att_share_for_submitted_att_body(dv, hn', att_share, a)
+    // ensures s'.bn.attestations_submitted == s.bn.attestations_submitted     
+    {
+        var activate_att_consensus_intances := process.attestation_consensus_engine_state.active_attestation_consensus_instances.Keys;
+
+        if pred_listen_for_attestation_shares_checker(
+                process,
+                attestation_share) 
+        {
+            var k := (attestation_share.data, attestation_share.aggregation_bits);
+            var process := f_add_new_attestation_share(
+                                    process,
+                                    attestation_share
+                                );
+
+                        
+            if process.construct_signed_attestation_signature(process.rcvd_attestation_shares[attestation_share.data.slot][k]).isPresent()
+            {
+                var aggregated_attestation := 
+                        Attestation(
+                            aggregation_bits := attestation_share.aggregation_bits,
+                            data := attestation_share.data,
+                            signature := process.construct_signed_attestation_signature(process.rcvd_attestation_shares[attestation_share.data.slot][k]).safe_get()
+                        );
+
+                var att_shares := process.rcvd_attestation_shares[attestation_share.data.slot][k];
+                assert construct_signed_attestation_signature_assumptions_helper_reverse(
+                    process.construct_signed_attestation_signature,
+                    process.dv_pubkey,
+                    dv.all_nodes                    
+                );
+
+                assert process.construct_signed_attestation_signature(att_shares).isPresent();
+
+                assert construct_signed_attestation_signature_assumptions_helper_reverse(
+                    process.construct_signed_attestation_signature,
+                    process.dv_pubkey,
+                    dv.all_nodes
+                );
+
+                var data: AttestationData :|
+                    construct_signed_attestation_signature_assumptions_helper_reverse_helper(
+                        process.construct_signed_attestation_signature,
+                        process.dv_pubkey,
+                        dv.all_nodes,
+                        att_shares,
+                        data                
+                    );
+
+                assert pred_rcvd_attestation_shares_is_in_all_messages_sent_single_node_state(dv, process);
+                assert att_shares <= dv.att_network.allMessagesSent;
+
+                var fork_version := bn_get_fork_version(compute_start_slot_at_epoch(data.target.epoch));
+                var signing_root := compute_attestation_signing_root(data, fork_version);
+
+
+                var signers := 
+                set signer, att_share | 
+                    && att_share in att_shares
+                    && signer in dv.all_nodes
+                    && verify_bls_siganture(signing_root, att_share.signature, signer)
+                ::
+                    signer;
+
+                assert signers <= dv.all_nodes;
+
+                lemmaThereExistsAnHonestInQuorum(dv.all_nodes, dv.all_nodes - dv.honest_nodes_states.Keys, signers);
+
+                var h_s :| h_s in dv.honest_nodes_states.Keys && h_s in signers;
+                var h_s_att :| h_s_att in att_shares && verify_bls_siganture(signing_root, h_s_att.signature, h_s);               
+
+                assert 
+                && h_s in dv.honest_nodes_states.Keys
+                && h_s_att in dv.att_network.allMessagesSent
+                && h_s_att.data == data
+                && verify_bls_siganture(signing_root, h_s_att.signature, h_s);
+
+                assert 
+                && h_s in dv.honest_nodes_states.Keys
+                && h_s_att in dv.att_network.allMessagesSent
+                && h_s_att.data == data
+                && verify_bls_siganture(signing_root, h_s_att.signature, h_s);
+
+                assert inv_exists_honest_dvc_that_sent_att_share_for_submitted_att_body(
+                    dv,
+                    h_s,
+                    h_s_att,
+                    aggregated_attestation
+                );
+
+                var state := f_add_new_submitted_attestation(process, aggregated_attestation);
+
+                forall a | a in state.bn.attestations_submitted 
+                {
+                    assert exists hn', att_share: AttestationShare :: inv_exists_honest_dvc_that_sent_att_share_for_submitted_att_body(dv, hn', att_share, a);
+                }
+                assert s' == state;
+            }
+        }   
+    }
+
+    // TODO: simplify this proof
+    lemma lem_inv_exists_honest_dvc_that_sent_att_share_for_submitted_att_ex_f_listen_for_attestation_shares(
+        process: DVCState,
+        attestation_share: AttestationShare,
+
+        s': DVCState,
+        dv: DVState
+    )
+    requires f_listen_for_attestation_shares.requires(process, attestation_share)
+    requires s' == f_listen_for_attestation_shares(process, attestation_share).state
+    requires construct_signed_attestation_signature_assumptions_helper(
+        process.construct_signed_attestation_signature,
+        process.dv_pubkey,
+        dv.all_nodes
+    )
+    requires inv_quorum_constraints(dv)
+    requires attestation_share in dv.att_network.allMessagesSent
+    requires pred_rcvd_attestation_shares_is_in_all_messages_sent_single_node_state(dv, process)
+    ensures forall a | a in f_listen_for_attestation_shares(process, attestation_share).outputs.attestations_submitted ::
+                        exists hn', att_share: AttestationShare :: inv_exists_honest_dvc_that_sent_att_share_for_submitted_att_body(dv, hn', att_share, a);
+    {
+        var activate_att_consensus_intances := process.attestation_consensus_engine_state.active_attestation_consensus_instances.Keys;
+
+        if pred_listen_for_attestation_shares_checker(
+                process,
+                attestation_share) 
+        {
+            var k := (attestation_share.data, attestation_share.aggregation_bits);
+            var process := f_add_new_attestation_share(
+                        process,
+                        attestation_share
+                    );
+                        
+            if process.construct_signed_attestation_signature(process.rcvd_attestation_shares[attestation_share.data.slot][k]).isPresent()
+            {
+                var aggregated_attestation := 
+                        Attestation(
+                            aggregation_bits := attestation_share.aggregation_bits,
+                            data := attestation_share.data,
+                            signature := process.construct_signed_attestation_signature(process.rcvd_attestation_shares[attestation_share.data.slot][k]).safe_get()
+                        );
+
+                var att_shares := process.rcvd_attestation_shares[attestation_share.data.slot][k];
+                assert construct_signed_attestation_signature_assumptions_helper_reverse(
+                    process.construct_signed_attestation_signature,
+                    process.dv_pubkey,
+                    dv.all_nodes                    
+                );
+
+                assert process.construct_signed_attestation_signature(att_shares).isPresent();
+
+                assert construct_signed_attestation_signature_assumptions_helper_reverse(
+                    process.construct_signed_attestation_signature,
+                    process.dv_pubkey,
+                    dv.all_nodes
+                );
+
+                var data: AttestationData :|
+                    construct_signed_attestation_signature_assumptions_helper_reverse_helper(
+                        process.construct_signed_attestation_signature,
+                        process.dv_pubkey,
+                        dv.all_nodes,
+                        att_shares,
+                        data                
+                    );
+
+                var fork_version := bn_get_fork_version(compute_start_slot_at_epoch(data.target.epoch));
+                var signing_root := compute_attestation_signing_root(data, fork_version);
+
+
+                var signers := 
+                set signer, att_share | 
+                    && att_share in att_shares
+                    && signer in dv.all_nodes
+                    && verify_bls_siganture(signing_root, att_share.signature, signer)
+                ::
+                    signer;
+
+                assert signers <= dv.all_nodes;
+
+                lemmaThereExistsAnHonestInQuorum(dv.all_nodes, dv.all_nodes - dv.honest_nodes_states.Keys, signers);
+
+                var h_s :| h_s in dv.honest_nodes_states.Keys && h_s in signers;
+                var h_s_att :| h_s_att in att_shares && verify_bls_siganture(signing_root, h_s_att.signature, h_s);
+        
+                assert  && h_s in dv.honest_nodes_states.Keys
+                        && h_s_att in dv.att_network.allMessagesSent
+                        && h_s_att.data == data
+                        && verify_bls_siganture(signing_root, h_s_att.signature, h_s);
+
+                assert  && h_s in dv.honest_nodes_states.Keys
+                        && h_s_att in dv.att_network.allMessagesSent
+                        && h_s_att.data == data
+                        && verify_bls_siganture(signing_root, h_s_att.signature, h_s);
+
+                assert inv_exists_honest_dvc_that_sent_att_share_for_submitted_att_body(
+                                dv,
+                                h_s,
+                                h_s_att,
+                                aggregated_attestation
+                            );
+
+                assert f_listen_for_attestation_shares(process, attestation_share).outputs.attestations_submitted == {aggregated_attestation};
+
+                assert forall a | a in f_listen_for_attestation_shares(process, attestation_share).outputs.attestations_submitted ::
+                            exists hn', att_share: AttestationShare :: inv_exists_honest_dvc_that_sent_att_share_for_submitted_att_body(dv, hn', att_share, a);
+            }
+        }   
+    }    
+
+    lemma lem_pred_rcvd_attestation_shares_is_in_all_messages_sent_f_listen_for_attestation_shares(
+        process: DVCState,
+        attestation_share: AttestationShare,
+        s': DVCState,
+        dv: DVState
+    )
+    requires f_listen_for_attestation_shares.requires(process, attestation_share)
+    requires s' == f_listen_for_attestation_shares(process, attestation_share).state
+    requires pred_rcvd_attestation_shares_is_in_all_messages_sent_single_node_state(dv, process)
+    requires attestation_share in dv.att_network.allMessagesSent
+    ensures pred_rcvd_attestation_shares_is_in_all_messages_sent_single_node_state(dv, s') 
+    { }    
+
+    lemma lem_inv_exists_honest_dvc_that_sent_att_share_for_submitted_att_ex_helper(
+        s: DVState,
+        event: DV.Event,
+        s': DVState
+    )
+    requires NextEventPreCond(s, event)
+    requires NextEvent(s, event, s')  
+    requires inv_exists_honest_dvc_that_sent_att_share_for_submitted_att(s)
+    requires s'.all_attestations_created == s.all_attestations_created
+    ensures inv_exists_honest_dvc_that_sent_att_share_for_submitted_att(s');
+    {
+        forall a |
+            && a in s'.all_attestations_created
+            && is_valid_attestation(a, s'.dv_pubkey)
+        ensures exists hn', att_share: AttestationShare :: inv_exists_honest_dvc_that_sent_att_share_for_submitted_att_body(s', hn', att_share, a);
+        {
+            var hn', att_share: AttestationShare :|
+                inv_exists_honest_dvc_that_sent_att_share_for_submitted_att_body(s, hn', att_share, a);
+            
+            assert inv_exists_honest_dvc_that_sent_att_share_for_submitted_att_body(s', hn', att_share, a);
+            assert exists hn', att_share: AttestationShare :: inv_exists_honest_dvc_that_sent_att_share_for_submitted_att_body(s', hn', att_share, a);
+        }
+    }    
+
+    // // 1m 10s
+    // TODO: simplify this lemma
+    lemma lem_inv_exists_honest_dvc_that_sent_att_share_for_submitted_att(
+        s: DVState,
+        event: DV.Event,
+        s': DVState
+    )
+    requires NextEventPreCond(s, event)
+    requires NextEvent(s, event, s')  
+    requires inv_exists_honest_dvc_that_sent_att_share_for_submitted_att(s)
+    requires construct_signed_attestation_signature_assumptions_helper(
+        s.construct_signed_attestation_signature,
+        s.dv_pubkey,
+        s.all_nodes
+    )
+    requires inv_only_dv_construct_signed_attestation_signature(s)  
+    requires invNetwork(s)
+    requires inv_quorum_constraints(s)
+    requires pred_rcvd_attestation_shares_is_in_all_messages_sent(s)    
+    ensures inv_exists_honest_dvc_that_sent_att_share_for_submitted_att(s')
+    {
+        assert s.att_network.allMessagesSent <= s'.att_network.allMessagesSent;
+        match event 
+        {
+            case HonestNodeTakingStep(node, nodeEvent, nodeOutputs) =>
+                var s_node := s.honest_nodes_states[node];
+                var s'_node := s'.honest_nodes_states[node];
+                match nodeEvent
+                {
+                    case ServeAttstationDuty(attestation_duty) => 
+                        lem_inv_exists_honest_dvc_that_sent_att_share_for_submitted_att_ex_helper(s, event, s');
+                        assert inv_exists_honest_dvc_that_sent_att_share_for_submitted_att(s');  
+
+                    case AttConsensusDecided(id, decided_attestation_data) => 
+                        lem_f_att_consensus_decided_unchanged_dvc_vars(s.honest_nodes_states[node], id, decided_attestation_data, s'.honest_nodes_states[node]);
+                        lem_inv_exists_honest_dvc_that_sent_att_share_for_submitted_att_ex_helper(s, event, s');
+                        assert inv_exists_honest_dvc_that_sent_att_share_for_submitted_att(s');            
+
+                    case ReceivedAttestationShare(attestation_share) => 
+                        assert multiset(addReceipientToMessages<AttestationShare>({attestation_share}, node)) <= s.att_network.messagesInTransit;
+
+                        assert MessaageWithRecipient(message := attestation_share, receipient := node) in s.att_network.messagesInTransit;      
+
+                        var stateAndOutput := f_listen_for_attestation_shares(s_node, attestation_share);  
+
+                        
+                        assert attestation_share in s.att_network.allMessagesSent;
+                        assert s'.all_attestations_created == s.all_attestations_created + stateAndOutput.outputs.attestations_submitted;
+
+                        lem_inv_exists_honest_dvc_that_sent_att_share_for_submitted_att_ex_f_listen_for_attestation_shares(
+                            s_node,
+                            attestation_share,
+                            s'_node,
+                            s
+                        );
+
+                        forall a | 
+                                    && a in s'.all_attestations_created
+                                    && is_valid_attestation(a, s'.dv_pubkey)
+                        ensures exists hn', att_share: AttestationShare :: inv_exists_honest_dvc_that_sent_att_share_for_submitted_att_body(s', hn', att_share, a);            
+                        {
+                            if a in s.all_attestations_created
+                            {
+                                var hn', att_share: AttestationShare :| inv_exists_honest_dvc_that_sent_att_share_for_submitted_att_body(s, hn', att_share, a);
+                                assert inv_exists_honest_dvc_that_sent_att_share_for_submitted_att_body(s', hn', att_share, a);
+                            }
+                            else 
+                            {
+                                assert a in stateAndOutput.outputs.attestations_submitted;
+                                var hn', att_share: AttestationShare :| inv_exists_honest_dvc_that_sent_att_share_for_submitted_att_body(s, hn', att_share, a);
+                                assert inv_exists_honest_dvc_that_sent_att_share_for_submitted_att_body(s', hn', att_share, a);
+                            }                                   
+                        }                                
+
+                        assert inv_exists_honest_dvc_that_sent_att_share_for_submitted_att(s');         
+
+                    case ImportedNewBlock(block) => 
+                        var s_node := f_add_block_to_bn(s_node, nodeEvent.block);
+                        lem_f_listen_for_new_imported_blocksd_unchanged_dvc_vars(s_node, block, s'_node);
+                        assert s'.all_attestations_created == s.all_attestations_created;
+                        lem_inv_exists_honest_dvc_that_sent_att_share_for_submitted_att_ex_helper(s, event, s');
+                        assert inv_exists_honest_dvc_that_sent_att_share_for_submitted_att(s');     
+
+                    case ResendAttestationShares => 
+                        assert s'.all_attestations_created == s.all_attestations_created;
+                        lem_inv_exists_honest_dvc_that_sent_att_share_for_submitted_att_ex_helper(s, event, s');
+                        assert inv_exists_honest_dvc_that_sent_att_share_for_submitted_att(s');
+
+                    case NoEvent => 
+                        assert s'.all_attestations_created == s.all_attestations_created;
+                        lem_inv_exists_honest_dvc_that_sent_att_share_for_submitted_att_ex_helper(s, event, s');
+                        assert inv_exists_honest_dvc_that_sent_att_share_for_submitted_att(s');
+                }
+
+            case AdeversaryTakingStep(node, new_attestation_share_sent, messagesReceivedByTheNode) =>
+                forall a | 
+                    && a in s'.all_attestations_created
+                    && is_valid_attestation(a, s'.dv_pubkey)
+                ensures exists hn', att_share: AttestationShare :: inv_exists_honest_dvc_that_sent_att_share_for_submitted_att_body(s', hn', att_share, a);      
+                {
+                    if a in s.all_attestations_created
+                    {
+                        var hn', att_share: AttestationShare :| inv_exists_honest_dvc_that_sent_att_share_for_submitted_att_body(s, hn', att_share, a);
+                        assert inv_exists_honest_dvc_that_sent_att_share_for_submitted_att_body(s', hn', att_share, a);                        
+                    }
+                    else 
+                    {
+                        var attestation_shares :| 
+                            && attestation_shares <= s'.att_network.allMessagesSent
+                            // && var sig_shares := set x | x in attestation_shares :: x.signature;
+                            && var constructed_sig := s.construct_signed_attestation_signature(attestation_shares);
+                            && constructed_sig.isPresent()
+                            && constructed_sig.safe_get() == a.signature
+                            ;      
+
+                        var constructed_sig := s.construct_signed_attestation_signature(attestation_shares);         
+
+                        var data: AttestationData :|
+                            construct_signed_attestation_signature_assumptions_helper_reverse_helper(
+                                s.construct_signed_attestation_signature,
+                                s.dv_pubkey,
+                                s.all_nodes,
+                                attestation_shares,
+                                data                
+                            );   
+
+                        var fork_version := bn_get_fork_version(compute_start_slot_at_epoch(data.target.epoch));
+                        var signing_root := compute_attestation_signing_root(data, fork_version);
+    
+
+                        var signers := 
+                        set signer, att_share | 
+                            && att_share in attestation_shares
+                            && signer in s.all_nodes
+                            && verify_bls_siganture(signing_root, att_share.signature, signer)
+                        ::
+                            signer;            
+
+                        assert signers <= s.all_nodes;
+
+                        lemmaThereExistsAnHonestInQuorum(s.all_nodes, s.all_nodes - s.honest_nodes_states.Keys, signers);  
+
+                        var h_s :| h_s in s.honest_nodes_states.Keys && h_s in signers;
+                        var h_s_att :| h_s_att in attestation_shares && verify_bls_siganture(signing_root, h_s_att.signature, h_s);     
+
+                        assert 
+                        && h_s in s.honest_nodes_states.Keys
+                        && h_s_att in s.att_network.allMessagesSent
+                        && h_s_att.data == data
+                        && verify_bls_siganture(signing_root, h_s_att.signature, h_s);
+
+                        assert 
+                        && h_s in s.honest_nodes_states.Keys
+                        && h_s_att in s.att_network.allMessagesSent
+                        && h_s_att.data == data
+                        && verify_bls_siganture(signing_root, h_s_att.signature, h_s);    
+
+                        compute_signing_root_properties<AttestationData>();
+                        lem_verify_bls_siganture();
+
+                        var a_fork_version := bn_get_fork_version(compute_start_slot_at_epoch(a.data.target.epoch));
+                        var a_attestation_signing_root := compute_attestation_signing_root(a.data, a_fork_version);       
+
+                        assert verify_bls_siganture(signing_root, a.signature, s'.dv_pubkey);
+
+                        assert verify_bls_siganture(a_attestation_signing_root, a.signature, s'.dv_pubkey);             
+
+                        // assert 
+
+                        assert inv_exists_honest_dvc_that_sent_att_share_for_submitted_att_body(
+                            s,
+                            h_s,
+                            h_s_att,
+                            a
+                        );      
+
+                        assert inv_exists_honest_dvc_that_sent_att_share_for_submitted_att_body(
+                            s',
+                            h_s,
+                            h_s_att,
+                            a
+                        );                                                                                                                                                 
+                    }
+                }
+                assert inv_exists_honest_dvc_that_sent_att_share_for_submitted_att(s');
+        }
+    }        
+
+    lemma lem_pred_rcvd_attestation_shares_is_in_all_messages_sent(
+        s: DVState,
+        event: DV.Event,
+        s': DVState
+    )
+    requires NextEventPreCond(s, event)
+    requires NextEvent(s, event, s')  
+    requires invNetwork(s)
+    requires pred_rcvd_attestation_shares_is_in_all_messages_sent(s)
+    ensures pred_rcvd_attestation_shares_is_in_all_messages_sent(s')
+    {
+        match event 
+        {
+            case HonestNodeTakingStep(node, nodeEvent, nodeOutputs) =>
+                var s_node := s.honest_nodes_states[node];
+                var s'_node := s'.honest_nodes_states[node];
+                match nodeEvent
+                {
+                    case ServeAttstationDuty(attestation_duty) => 
+                        lem_f_serve_attestation_duty_constants(s_node, attestation_duty, s'_node);
+
+                    case AttConsensusDecided(id, decided_attestation_data) => 
+                        lem_f_att_consensus_decided_unchanged_dvc_vars(s_node, id, decided_attestation_data, s'_node);
+
+                    case ReceivedAttestationShare(attestation_share) => 
+                        assert multiset(addReceipientToMessages<AttestationShare>({attestation_share}, node)) <= s.att_network.messagesInTransit;
+                        assert MessaageWithRecipient(message := attestation_share, receipient := node) in s.att_network.messagesInTransit;        
+                        assert attestation_share in s.att_network.allMessagesSent;                    
+                        lem_pred_rcvd_attestation_shares_is_in_all_messages_sent_f_listen_for_attestation_shares(
+                            s_node,
+                            attestation_share,
+                            s'_node,
+                            s
+                        );
+
+                    case ImportedNewBlock(block) => 
+                        var s_node := f_add_block_to_bn(s_node, nodeEvent.block);
+                        lem_f_listen_for_new_imported_blocksd_unchanged_dvc_vars(s_node, block, s'_node);
+                        assert pred_rcvd_attestation_shares_is_in_all_messages_sent(s');      
+
+                    case ResendAttestationShares => 
+                        assert pred_rcvd_attestation_shares_is_in_all_messages_sent(s');                    
+                    case NoEvent => 
+
+                }
+
+            case AdeversaryTakingStep(node, new_attestation_share_sent, messagesReceivedByTheNode) =>
+
+        }
+    }     
+
+    lemma lem_getMessagesFromEmptySetOfMessagesWithRecipient_is_empty_set<M>(mswr: set<MessaageWithRecipient<M>>)
+    requires mswr == {}
+    ensures getMessagesFromMessagesWithRecipient(mswr) == {}
+    {
+    }
+
+    // TODO
+    lemma lem_inv_data_of_att_share_is_decided_value_helper(
+        s: DVState,
+        event: DV.Event,
+        s': DVState
+    )
+    requires NextEventPreCond(s, event)
+    requires NextEvent(s, event, s')  
+    requires inv_data_of_att_share_is_decided_value(s)
+    requires inv_decided_value_of_consensus_instance_of_slot_k_is_for_slot_k(s)
+    requires inv_quorum_constraints(s)
+    requires same_honest_nodes_in_dv_and_ci(s)
+    requires inv_only_dv_construct_signed_attestation_signature(s)
+    requires |s.all_nodes| > 0
+    requires s'.att_network.allMessagesSent == 
+                    s.att_network.allMessagesSent + getMessagesFromMessagesWithRecipient({});
+    ensures  inv_data_of_att_share_is_decided_value(s');
+    {
+        forall cid | cid in s.consensus_on_attestation_data.Keys 
+        ensures && var s_consensus := s.consensus_on_attestation_data[cid];
+                && var s'_consensus := s'.consensus_on_attestation_data[cid];
+                && s_consensus.decided_value.isPresent() ==> 
+                        ( && s'_consensus.decided_value.isPresent()
+                          && s_consensus.decided_value.safe_get() == s'_consensus.decided_value.safe_get()
+                        )
+            ;
+        {
+            var s_consensus := s.consensus_on_attestation_data[cid];
+            var s'_consensus := s'.consensus_on_attestation_data[cid];
+
+            assert isConditionForSafetyTrue(s_consensus);
+            assert s_consensus.decided_value.isPresent() ==> 
+                && s'_consensus.decided_value.isPresent()
+                && s_consensus.decided_value.safe_get() == s'_consensus.decided_value.safe_get()
+            ;
+        }
+
+        assert forall cid | cid in s.consensus_on_attestation_data.Keys :: 
+                    && var s_consensus := s.consensus_on_attestation_data[cid];
+                    && var s'_consensus := s'.consensus_on_attestation_data[cid];
+                    && s_consensus.decided_value.isPresent() ==> 
+                            ( && s'_consensus.decided_value.isPresent()
+                            && s_consensus.decided_value.safe_get() == s'_consensus.decided_value.safe_get()
+                            )
+        ;
+
+        var emptySet: set<MessaageWithRecipient<AttestationShare>> := {};
+        calc {
+            s'.att_network.allMessagesSent;
+            == 
+            s.att_network.allMessagesSent + getMessagesFromMessagesWithRecipient(emptySet);
+            ==
+            {lem_getMessagesFromEmptySetOfMessagesWithRecipient_is_empty_set(emptySet);}
+            s.att_network.allMessagesSent;
+        }
+
+        assert s'.att_network.allMessagesSent == s.att_network.allMessagesSent;        
+
+        forall hn, att_share |
+                && hn in s'.honest_nodes_states.Keys 
+                && att_share in s'.att_network.allMessagesSent
+                && var fork_version := bn_get_fork_version(compute_start_slot_at_epoch(att_share.data.target.epoch));                
+                && var attestation_signing_root := compute_attestation_signing_root(att_share.data, fork_version);
+                && verify_bls_siganture(attestation_signing_root, att_share.signature, hn)
+        ensures inv_data_of_att_share_is_decided_value_body(s', att_share);
+        {
+            assert att_share in s.att_network.allMessagesSent;
+            assert inv_data_of_att_share_is_decided_value_body(s, att_share);
+            assert inv_data_of_att_share_is_decided_value_body(s', att_share);
+        }
+
+        assert inv_data_of_att_share_is_decided_value(s');   
+    }     
+
+    lemma lem_consensus_next_under_safety<D(!new, 0)>(
+        s: ConsensusInstance,
+        honest_nodes_validity_predicates: map<BLSPubkey, D -> bool>,        
+        s': ConsensusInstance,
+        output: Optional<OutCommand>
+    )
+    requires ConsensusSpec.Next(s, honest_nodes_validity_predicates, s', output)
+    requires isConditionForSafetyTrue(s)
+    requires s.decided_value.isPresent()
+    ensures s'.decided_value.isPresent()
+    ensures s.decided_value.safe_get() == s'.decided_value.safe_get()
+    { }
 
     
-    lemma lem_inv_all_in_transit_messages_were_sent_dv_next(
-        dv: DVState,
-        event: DV.Event,
-        dv': DVState
-    )    
-    requires NextEventPreCond(dv, event)
-    requires NextEvent(dv, event, dv')    
-    requires inv_all_in_transit_messages_were_sent(dv)
-    ensures inv_all_in_transit_messages_were_sent(dv')    
-    {
-        var n: BLSPubkey,
-            messagesToBeSent: set<MessaageWithRecipient<AttestationShare>>,
-            messagesReceived: set<AttestationShare> 
-            :|
-            NetworkSpec.Next<AttestationShare>(
-                dv.att_network, 
-                dv'.att_network, 
-                n, 
-                messagesToBeSent, 
-                messagesReceived);
 
-        lem_inv_all_in_transit_messages_were_sent_body_network_spec_next<AttestationShare>(
-                dv.att_network, 
-                dv'.att_network, 
-                n, 
-                messagesToBeSent, 
-                messagesReceived);  
+    lemma lem_inv_sent_validity_predicate_is_based_on_rcvd_att_duty_and_slashing_db_get_s_w_honest_node_states_updated(
+        s: DVState,
+        node: BLSPubkey,
+        nodeEvent: Types.Event
+    ) returns (s_w_honest_node_states_updated: DVState)
+    requires node in s.honest_nodes_states
+    ensures s_w_honest_node_states_updated == add_block_to_bn_with_event(s, node, nodeEvent)
+    ensures s_w_honest_node_states_updated == s.(honest_nodes_states := s_w_honest_node_states_updated.honest_nodes_states)
+    ensures s_w_honest_node_states_updated.honest_nodes_states == s.honest_nodes_states[node := s_w_honest_node_states_updated.honest_nodes_states[node]]
+    ensures s_w_honest_node_states_updated.honest_nodes_states[node] == s.honest_nodes_states[node].(bn := s_w_honest_node_states_updated.honest_nodes_states[node].bn)
+    {
+        s_w_honest_node_states_updated :=
+            if nodeEvent.ImportedNewBlock? then 
+                s.(
+                    honest_nodes_states := s.honest_nodes_states[node := f_add_block_to_bn(s.honest_nodes_states[node], nodeEvent.block)]
+                )
+            else 
+                s 
+            ;         
     }
 
-    lemma lem_inv_all_in_transit_messages_were_sent_invNetwork(dv: DVState)
-    requires inv_all_in_transit_messages_were_sent(dv)
-    ensures invNetwork(dv)
-    {}
+    lemma  lemmaNextConsensus<D(!new, 0)>(
+        s: ConsensusInstance,
+        honest_nodes_validity_predicates: map<BLSPubkey, D -> bool>,        
+        s': ConsensusInstance,
+        output: Optional<OutCommand>
+    )
+    requires ConsensusSpec.Next(
+                        s,
+                        honest_nodes_validity_predicates,
+                        s',
+                        output
+                    );
+    ensures s.honest_nodes_validity_functions.Keys <= s'.honest_nodes_validity_functions.Keys;                 
+    {
+    }
 
-    lemma lem_inv_attestation_shares_to_broadcast_are_sent_messages_dv_next(
-        dv: DVState,
+    lemma  lemmaNextConsensus2<D(!new, 0)>(
+        s: ConsensusInstance,
+        honest_nodes_validity_predicates: map<BLSPubkey, D -> bool>,        
+        s': ConsensusInstance,
+        output: Optional<OutCommand>,
+        n: BLSPubkey
+    )
+    requires ConsensusSpec.Next(
+                        s,
+                        honest_nodes_validity_predicates,
+                        s',
+                        output
+                    );
+    requires n in s.honest_nodes_validity_functions.Keys
+    ensures s.honest_nodes_validity_functions[n] <= s'.honest_nodes_validity_functions[n];                    
+    {
+    }   
+
+    lemma lem_inv_data_of_att_share_is_decided_value_att_consensus_decided_helper_2(
+        s: DVState,
         event: DV.Event,
-        dv': DVState
-    )       
-    requires NextEventPreCond(dv, event)
-    requires NextEvent(dv, event, dv')  
-    requires inv_quorum_constraints(dv)
-    requires inv_unchanged_honesty(dv)
-    requires inv_only_dv_construct_signed_attestation_signature(dv)
-    requires same_honest_nodes_in_dv_and_ci(dv)    
-    requires inv_decided_value_of_consensus_instance_is_decided_by_quorum(dv)    
-    requires inv_sent_validity_predicate_is_based_on_rcvd_att_duty_and_slashing_db(dv)
-    requires inv_sent_validity_predicate_is_based_on_rcvd_att_duty_and_slashing_db_for_dv(dv)      
-    requires inv_decided_value_of_consensus_instance_of_slot_k_is_for_slot_k(dv)       
-    requires inv_attestation_shares_to_broadcast_are_sent_messages(dv)    
-    ensures inv_attestation_shares_to_broadcast_are_sent_messages(dv')
-    {   
-        lem_inv_quorum_constraints_dv_next(dv, event, dv');
-        lem_inv_unchanged_honesty_dv_next(dv, event, dv');
-        lem_inv_only_dv_construct_signed_attestation_signature_dv_next(dv, event, dv');
-
-        assert && inv_quorum_constraints(dv')
-               && inv_unchanged_honesty(dv')
-               && inv_only_dv_construct_signed_attestation_signature(dv');
-        
-
+        s': DVState
+    )
+    requires NextEventPreCond(s, event)
+    requires NextEvent(s, event, s')  
+    requires event.HonestNodeTakingStep?
+    requires event.event.AttConsensusDecided?
+    requires inv_quorum_constraints(s)
+    requires inv_unchanged_honesty(s)        
+    requires |s.all_nodes| > 0    
+    ensures s'.consensus_on_attestation_data[event.event.id].decided_value.safe_get() == event.event.decided_attestation_data; 
+    {
         match event 
         {
             case HonestNodeTakingStep(node, nodeEvent, nodeOutputs) =>
-                var dvc := dv.honest_nodes_states[node];
-                var dvc' := dv'.honest_nodes_states[node];
-                assert && dvc.peers == dvc'.peers
-                       && |dvc.peers| > 0 ;
-
+                var s_node := s.honest_nodes_states[node];
+                var s'_node := s'.honest_nodes_states[node];
                 match nodeEvent
                 {
-                    case ServeAttstationDuty(att_duty) =>     
-                        lem_inv_attestation_shares_to_broadcast_are_sent_messages_f_serve_attestation_duty(dvc, att_duty, dvc');                        
-                        
-                    case AttConsensusDecided(id, decided_attestation_data) => 
-                        var att_network := dv.att_network;
-                        var att_network' := dv'.att_network;
-                        if id == decided_attestation_data.slot
-                        {
-                            lem_inv_attestation_shares_to_broadcast_are_sent_messages_f_att_consensus_decided(dvc, id, decided_attestation_data, dvc', nodeOutputs);   
-                            assert att_network'.allMessagesSent
-                                        == att_network.allMessagesSent + getMessagesFromMessagesWithRecipient(nodeOutputs.att_shares_sent);               
-                        }
-                                                
-                    case ReceivedAttestationShare(attestation_share) =>                         
-                        lem_inv_attestation_shares_to_broadcast_are_sent_messages_f_listen_for_attestation_shares(dvc, attestation_share, dvc');                                                
+                    case AttConsensusDecided(id: Slot, decided_attestation_data) => 
+                        var s_w_honest_node_states_updated := lem_inv_sent_validity_predicate_is_based_on_rcvd_att_duty_and_slashing_db_get_s_w_honest_node_states_updated(s, node, nodeEvent);           
+                        var cid := id;
 
-                    case ImportedNewBlock(block) => 
-                        var dvc_mod := f_add_block_to_bn(dvc, block);
-                        lem_inv_attestation_shares_to_broadcast_are_sent_messages_add_block_to_bn(dvc, block, dvc_mod);
-                        lem_inv_attestation_shares_to_broadcast_are_sent_messages_f_listen_for_new_imported_blocks(dvc_mod, block, dvc');                                                
-                                                
-                    case ResendAttestationShares =>                         
-                        lem_inv_attestation_shares_to_broadcast_are_sent_messages_f_resend_attestation_share(dvc, dvc');
+                        assert s_w_honest_node_states_updated.consensus_on_attestation_data == s.consensus_on_attestation_data;
 
-                    case NoEvent => 
-                        
+                        var output := Some(Decided(node, nodeEvent.decided_attestation_data)); 
+
+                        var validityPredicates := 
+                                map n |
+                                        && n in s_w_honest_node_states_updated.honest_nodes_states.Keys 
+                                        && cid in s_w_honest_node_states_updated.honest_nodes_states[n].attestation_consensus_engine_state.active_attestation_consensus_instances.Keys
+                                    ::
+                                        s_w_honest_node_states_updated.honest_nodes_states[n].attestation_consensus_engine_state.active_attestation_consensus_instances[cid].validityPredicate
+                                ;
+
+                        var s_consensus := s_w_honest_node_states_updated.consensus_on_attestation_data[cid];
+                        var s'_consensus := s'.consensus_on_attestation_data[cid];                
+
+                        assert ConsensusSpec.Next(
+                                    s_consensus,
+                                    validityPredicates,
+                                    s'_consensus,
+                                    output
+                                );                               
+
+                        assert s'.consensus_on_attestation_data[id].decided_value.isPresent();
+                        assert isConditionForSafetyTrue(s'_consensus);
+                        assert s'_consensus.decided_value.safe_get() == decided_attestation_data; 
+                        assert s'.consensus_on_attestation_data[id].decided_value.safe_get() == decided_attestation_data; 
+                }
+        }            
+    }
+
+    // // 1m 15s
+    lemma lem_inv_decided_value_of_consensus_instance_is_decided_by_quorum_helper(
+        s: DVState,
+        event: DV.Event,
+        cid: Slot,
+        s': DVState
+    )
+    requires NextEventPreCond(s, event)
+    requires NextEvent(s, event, s')  
+    requires event.HonestNodeTakingStep?
+    requires cid in s'.consensus_on_attestation_data.Keys
+    requires inv_quorum_constraints(s)
+    requires same_honest_nodes_in_dv_and_ci(s)
+    requires inv_only_dv_construct_signed_attestation_signature(s)
+    requires inv_decided_value_of_consensus_instance_is_decided_by_quorum(s)    
+    requires s.consensus_on_attestation_data[cid].decided_value.isPresent()
+    ensures is_a_valid_decided_value(s'.consensus_on_attestation_data[cid]); 
+    {
+        assert s.att_network.allMessagesSent <= s'.att_network.allMessagesSent;
+        match event 
+        {
+            case HonestNodeTakingStep(node, nodeEvent, nodeOutputs) =>
+                var s_node := s.honest_nodes_states[node];
+                var s'_node := s'.honest_nodes_states[node];
+
+                var s_w_honest_node_states_updated :=
+                    if nodeEvent.ImportedNewBlock? then 
+                        s.(
+                            honest_nodes_states := s.honest_nodes_states[node := f_add_block_to_bn(s.honest_nodes_states[node], nodeEvent.block)]
+                        )
+                    else 
+                        s 
+                    ;                
+
+                assert s_w_honest_node_states_updated.consensus_on_attestation_data == s.consensus_on_attestation_data;
+
+
+                var output := 
+                    if nodeEvent.AttConsensusDecided? && nodeEvent.id == cid then 
+                        Some(Decided(node, nodeEvent.decided_attestation_data))
+                    else
+                        None
+                    ;
+
+                var validityPredicates := 
+                    map n |
+                            && n in s_w_honest_node_states_updated.honest_nodes_states.Keys 
+                            && cid in s_w_honest_node_states_updated.honest_nodes_states[n].attestation_consensus_engine_state.active_attestation_consensus_instances.Keys
+                        ::
+                            s_w_honest_node_states_updated.honest_nodes_states[n].attestation_consensus_engine_state.active_attestation_consensus_instances[cid].validityPredicate
+                    ;
+
+                var s_consensus := s_w_honest_node_states_updated.consensus_on_attestation_data[cid];
+                var s'_consensus := s'.consensus_on_attestation_data[cid];                
+
+                assert
+                    ConsensusSpec.Next(
+                        s_consensus,
+                        validityPredicates,
+                        s'_consensus,
+                        output
+                    );
+
+                
+                assert isConditionForSafetyTrue(s_consensus);
+                assert && s'_consensus.decided_value.isPresent()
+                       && s_consensus.decided_value.safe_get() == s'_consensus.decided_value.safe_get()
+                       ;
+
+                var h_nodes :| is_a_valid_decided_value_according_to_set_of_nodes(s_consensus, h_nodes); 
+
+                assert s_consensus.honest_nodes_validity_functions.Keys <= s'_consensus.honest_nodes_validity_functions.Keys;
+                assert         
+                    && var byz := s'.all_nodes - s'_consensus.honest_nodes_status.Keys;
+                    |h_nodes| >= quorum(|s.all_nodes|) - |byz|;
+
+                lemmaNextConsensus(
+                    s_consensus,
+                    validityPredicates,
+                    s'_consensus,
+                    output                        
+                );
+
+
+                forall n | n in h_nodes 
+                ensures exists vp: AttestationData -> bool :: vp in s'_consensus.honest_nodes_validity_functions[n] && vp(s'_consensus.decided_value.safe_get());
+                {
+                    assert is_a_valid_decided_value(s_consensus); 
+                    var vp: AttestationData -> bool :| vp in s_consensus.honest_nodes_validity_functions[n] && vp(s_consensus.decided_value.safe_get()); 
+                    lemmaNextConsensus2(
+                        s_consensus,
+                        validityPredicates,
+                        s'_consensus,
+                        output,
+                        n                       
+                    );                        
+                    assert vp in  s'_consensus.honest_nodes_validity_functions[n]; 
+                    assert vp(s'_consensus.decided_value.safe_get());
+                    assert exists vp: AttestationData -> bool :: vp in s'_consensus.honest_nodes_validity_functions[n] && vp(s'_consensus.decided_value.safe_get());
                 }
 
-            case AdeversaryTakingStep(node, new_attestation_share_sent, messagesReceivedByTheNode) =>
-                
-        }        
-    }  
+                assert is_a_valid_decided_value_according_to_set_of_nodes(s'_consensus, h_nodes); 
+                assert is_a_valid_decided_value(s'_consensus); 
+        }
+    }   
 
-    // TODO: Rename
-    lemma lem_inv39_dv_next(
-        dv: DVState,
+    lemma lem_inv_decided_value_of_consensus_instance_is_decided_by_quorum(
+        s: DVState,
         event: DV.Event,
-        dv': DVState
-    )       
-    requires NextEventPreCond(dv, event)
-    requires NextEvent(dv, event, dv')  
-    ensures dv.att_network.allMessagesSent <= dv'.att_network.allMessagesSent
-    {}
-
-    lemma lem_inv_rcvd_attn_shares_are_from_sent_messages_dv_next(
-        dv: DVState,
-        event: DV.Event,
-        dv': DVState
-    )       
-    requires NextEventPreCond(dv, event)
-    requires NextEvent(dv, event, dv')  
-    requires inv_all_in_transit_messages_were_sent(dv)
-    requires inv_rcvd_attn_shares_are_from_sent_messages(dv)
-    ensures inv_rcvd_attn_shares_are_from_sent_messages(dv')
-    {        
+        s': DVState
+    )
+    requires NextEventPreCond(s, event)
+    requires NextEvent(s, event, s')  
+    requires inv_quorum_constraints(s)
+    requires same_honest_nodes_in_dv_and_ci(s)
+    requires inv_only_dv_construct_signed_attestation_signature(s)
+    requires inv_decided_value_of_consensus_instance_is_decided_by_quorum(s)    
+    ensures inv_decided_value_of_consensus_instance_is_decided_by_quorum(s')   
+    {
+        assert s.att_network.allMessagesSent <= s'.att_network.allMessagesSent;
         match event 
         {
             case HonestNodeTakingStep(node, nodeEvent, nodeOutputs) =>
-                var dvc := dv.honest_nodes_states[node];
-                var dvc' := dv'.honest_nodes_states[node];
+                var s_node := s.honest_nodes_states[node];
+                var s'_node := s'.honest_nodes_states[node];
+
+                var s_w_honest_node_states_updated :=
+                    if nodeEvent.ImportedNewBlock? then 
+                        s.(
+                            honest_nodes_states := s.honest_nodes_states[node := f_add_block_to_bn(s.honest_nodes_states[node], nodeEvent.block)]
+                        )
+                    else 
+                        s 
+                    ;                
+
+                forall cid | 
+                        && cid in s'.consensus_on_attestation_data.Keys
+                        && s'.consensus_on_attestation_data[cid].decided_value.isPresent()
+                ensures is_a_valid_decided_value(s'.consensus_on_attestation_data[cid]);
+                {
+                    if s.consensus_on_attestation_data[cid].decided_value.isPresent()
+                    {
+                        lem_inv_decided_value_of_consensus_instance_is_decided_by_quorum_helper(s, event, cid, s');
+                    }
+                    else
+                    {
+                        assert is_a_valid_decided_value(s'.consensus_on_attestation_data[cid]);
+                    }
+                }
+                assert inv_decided_value_of_consensus_instance_is_decided_by_quorum(s');
+               
+
+            case AdeversaryTakingStep(node, new_attestation_share_sent, messagesReceivedByTheNode) =>
+                assert inv_decided_value_of_consensus_instance_is_decided_by_quorum(s');
+        }        
+    } 
+
+    lemma lem_inv_decided_value_of_consensus_instance_of_slot_k_is_for_slot_k_helper(
+        s: DVState,
+        cid: Slot
+    )
+    requires inv_decided_value_of_consensus_instance_is_decided_by_quorum(s)    
+    requires inv_sent_validity_predicate_is_based_on_rcvd_att_duty_and_slashing_db(s)
+    requires inv_quorum_constraints(s)
+    requires inv_unchanged_honesty(s)
+    requires inv_only_dv_construct_signed_attestation_signature(s)
+    requires cid in s.consensus_on_attestation_data.Keys
+    requires s.consensus_on_attestation_data[cid].decided_value.isPresent()
+    ensures s.consensus_on_attestation_data[cid].decided_value.safe_get().slot == cid
+    {
+        var s_consensus := s.consensus_on_attestation_data[cid];
+        assert is_a_valid_decided_value(s_consensus);  
+
+        var h_nodes_a :| is_a_valid_decided_value_according_to_set_of_nodes(s_consensus, h_nodes_a);
+
+        var byz := s.all_nodes - s.honest_nodes_states.Keys;
+
+        assert byz * h_nodes_a == {} by 
+        {
+            assert s.honest_nodes_states.Keys * byz == {};
+        }
+
+        lemmaThereExistsAnHonestInQuorum2(s.all_nodes, byz, h_nodes_a);  
+
+        var h_n :| h_n in h_nodes_a;  
+
+        var vp: AttestationData -> bool :| vp in s_consensus.honest_nodes_validity_functions[h_n] && vp(s_consensus.decided_value.safe_get());  
+
+        var attestation_duty, attestation_slashing_db :|
+                inv_sent_validity_predicate_is_based_on_rcvd_att_duty_and_slashing_db_body(cid, attestation_duty, attestation_slashing_db, vp);
+
+        assert s_consensus.decided_value.safe_get().slot == cid;
+    }
+
+    lemma lem_inv_sent_validity_predicate_is_based_on_rcvd_att_duty_and_slashing_db_get_s_w_honest_node_states_updated_2(
+        s: DVState,
+        node: BLSPubkey,
+        nodeEvent: Types.Event,
+        node': BLSPubkey,
+        s_w_honest_node_states_updated: DVState
+    ) 
+    requires node in s.honest_nodes_states
+    requires node' in s.honest_nodes_states
+    requires s_w_honest_node_states_updated == add_block_to_bn_with_event(s, node, nodeEvent)
+    ensures s_w_honest_node_states_updated.honest_nodes_states[node'].attestation_consensus_engine_state == s.honest_nodes_states[node'].attestation_consensus_engine_state
+    {      
+    }  
+
+    lemma lem_inv_sent_validity_predicate_is_based_on_rcvd_att_duty_and_slashing_db_helper(
+        s: DVState,
+        event: DV.Event,
+        s': DVState,
+        cid: Slot,
+        hn: BLSPubkey,
+        vp: AttestationData -> bool
+    )   returns (attestation_duty: AttestationDuty, attestation_slashing_db: set<SlashingDBAttestation>)
+    requires NextEventPreCond(s, event)
+    requires NextEvent(s, event, s')    
+    requires inv_quorum_constraints(s)
+    requires inv_unchanged_honesty(s)
+    requires inv_only_dv_construct_signed_attestation_signature(s)      
+    requires
+            && hn in s'.consensus_on_attestation_data[cid].honest_nodes_validity_functions.Keys
+            && vp in s'.consensus_on_attestation_data[cid].honest_nodes_validity_functions[hn]
+    requires event.HonestNodeTakingStep?
+    requires inv_sent_validity_predicate_is_based_on_rcvd_att_duty_and_slashing_db(s)
+    requires inv_sent_validity_predicate_is_based_on_rcvd_att_duty_and_slashing_db_for_dv(s)
+    ensures inv_sent_validity_predicate_is_based_on_rcvd_att_duty_and_slashing_db_body(cid, attestation_duty, attestation_slashing_db, vp); 
+    {
+        assert s.att_network.allMessagesSent <= s'.att_network.allMessagesSent;
+        match event 
+        {
+            case HonestNodeTakingStep(node, nodeEvent, nodeOutputs) =>
+                var s_node := s.honest_nodes_states[node];
+                var s'_node := s'.honest_nodes_states[node];
+
+                var s_w_honest_node_states_updated :=
+                    lem_inv_sent_validity_predicate_is_based_on_rcvd_att_duty_and_slashing_db_get_s_w_honest_node_states_updated(s, node, nodeEvent);         
+
+                assert s_w_honest_node_states_updated.consensus_on_attestation_data == s.consensus_on_attestation_data;
+
+
+                var output := 
+                    if nodeEvent.AttConsensusDecided? && nodeEvent.id == cid then 
+                        Some(Decided(node, nodeEvent.decided_attestation_data))
+                    else
+                        None
+                    ;
+
+                var validityPredicates := 
+                    map n |
+                            && n in s_w_honest_node_states_updated.honest_nodes_states.Keys 
+                            && cid in s_w_honest_node_states_updated.honest_nodes_states[n].attestation_consensus_engine_state.active_attestation_consensus_instances.Keys
+                        ::
+                            s_w_honest_node_states_updated.honest_nodes_states[n].attestation_consensus_engine_state.active_attestation_consensus_instances[cid].validityPredicate
+                    ;
+
+                var s_consensus := s_w_honest_node_states_updated.consensus_on_attestation_data[cid];
+                var s'_consensus := s'.consensus_on_attestation_data[cid];                
+
+                assert
+                    ConsensusSpec.Next(
+                        s_consensus,
+                        validityPredicates,
+                        s'_consensus,
+                        output
+                    );
+
+            if hn in s_consensus.honest_nodes_validity_functions.Keys  && vp in s_consensus.honest_nodes_validity_functions[hn]
+            {
+                assert vp in s'_consensus.honest_nodes_validity_functions[hn];
+
+                attestation_duty, attestation_slashing_db :| inv_sent_validity_predicate_is_based_on_rcvd_att_duty_and_slashing_db_body(cid, attestation_duty, attestation_slashing_db, vp);
+
+            }
+            else 
+            {
+                assert vp in validityPredicates.Values;
+                var vpn :| vpn in validityPredicates.Keys && validityPredicates[vpn] == vp;
+                assert validityPredicates[vpn] == s_w_honest_node_states_updated.honest_nodes_states[vpn].attestation_consensus_engine_state.active_attestation_consensus_instances[cid].validityPredicate;
+
+                assert vpn in s.honest_nodes_states.Keys;
+                assert cid in s_w_honest_node_states_updated.honest_nodes_states[vpn].attestation_consensus_engine_state.active_attestation_consensus_instances.Keys;
+
+                lem_inv_sent_validity_predicate_is_based_on_rcvd_att_duty_and_slashing_db_get_s_w_honest_node_states_updated_2(s, node, nodeEvent, vpn, s_w_honest_node_states_updated);
+
+                assert s_w_honest_node_states_updated.honest_nodes_states[vpn].attestation_consensus_engine_state == s.honest_nodes_states[vpn].attestation_consensus_engine_state;
+                assert inv_sent_validity_predicate_is_based_on_rcvd_att_duty_and_slashing_db_for_dvc_single_dvc(s, vpn, cid);
+
+                attestation_duty, attestation_slashing_db :| inv_sent_validity_predicate_is_based_on_rcvd_att_duty_and_slashing_db_body(cid, attestation_duty, attestation_slashing_db, vp);
+            }
+
+            assert inv_sent_validity_predicate_is_based_on_rcvd_att_duty_and_slashing_db_body(cid, attestation_duty, attestation_slashing_db, vp);
+
+
+        }
+
+    }  
+
+    lemma lem_inv_sent_validity_predicate_is_based_on_rcvd_att_duty_and_slashing_db(
+        s: DVState,
+        event: DV.Event,
+        s': DVState
+    )   
+    requires NextEventPreCond(s, event)
+    requires NextEvent(s, event, s')    
+    requires inv_sent_validity_predicate_is_based_on_rcvd_att_duty_and_slashing_db(s)
+    requires inv_quorum_constraints(s)
+    requires inv_unchanged_honesty(s)
+    requires inv_only_dv_construct_signed_attestation_signature(s)      
+    requires inv_sent_validity_predicate_is_based_on_rcvd_att_duty_and_slashing_db_for_dv(s)  
+    ensures inv_sent_validity_predicate_is_based_on_rcvd_att_duty_and_slashing_db(s')   
+    {
+        match event 
+        {
+            case HonestNodeTakingStep(node, nodeEvent, nodeOutputs) =>
+                forall hn, cid: nat, vp |
+                    && hn in s'.consensus_on_attestation_data[cid].honest_nodes_validity_functions.Keys
+                    && vp in s'.consensus_on_attestation_data[cid].honest_nodes_validity_functions[hn]
+                ensures exists attestation_duty, attestation_slashing_db :: inv_sent_validity_predicate_is_based_on_rcvd_att_duty_and_slashing_db_body(cid, attestation_duty, attestation_slashing_db, vp)
+                {
+                    var attestation_duty: AttestationDuty, attestation_slashing_db := lem_inv_sent_validity_predicate_is_based_on_rcvd_att_duty_and_slashing_db_helper(s, event, s', cid, hn, vp);
+                }
+                assert inv_sent_validity_predicate_is_based_on_rcvd_att_duty_and_slashing_db(s');
+
+            case AdeversaryTakingStep(node, new_attestation_share_sent, messagesReceivedByTheNode) =>
+                assert inv_sent_validity_predicate_is_based_on_rcvd_att_duty_and_slashing_db(s');
+        }
+    }   
+
+    lemma lem_inv_decided_value_of_consensus_instance_of_slot_k_is_for_slot_k(
+        s: DVState,
+        event: DV.Event,
+        s': DVState
+    )
+    requires NextEventPreCond(s, event)
+    requires NextEvent(s, event, s')  
+    requires inv_decided_value_of_consensus_instance_is_decided_by_quorum(s)    
+    requires inv_sent_validity_predicate_is_based_on_rcvd_att_duty_and_slashing_db(s)
+    requires inv_sent_validity_predicate_is_based_on_rcvd_att_duty_and_slashing_db_for_dv(s)  
+    requires inv_quorum_constraints(s)
+    requires inv_unchanged_honesty(s)
+    requires inv_only_dv_construct_signed_attestation_signature(s)  
+    ensures inv_decided_value_of_consensus_instance_of_slot_k_is_for_slot_k(s') 
+    {
+        lem_inv_quorum_constraints_dv_next(s, event, s');
+        lem_inv_unchanged_honesty_dv_next(s, event, s');
+        lem_inv_only_dv_construct_signed_attestation_signature_dv_next(s, event, s');
+        lem_inv_decided_value_of_consensus_instance_is_decided_by_quorum(s, event, s');
+        lem_inv_sent_validity_predicate_is_based_on_rcvd_att_duty_and_slashing_db(s, event, s');
+        lem_inv_decided_value_of_consensus_instance_of_slot_k_is_for_slot_k2(s');   
+    }     
+
+    lemma lem_inv_decided_value_of_consensus_instance_of_slot_k_is_for_slot_k2(
+        s: DVState
+    )
+    requires inv_decided_value_of_consensus_instance_is_decided_by_quorum(s)    
+    requires inv_sent_validity_predicate_is_based_on_rcvd_att_duty_and_slashing_db(s)
+    requires inv_quorum_constraints(s)
+    requires inv_unchanged_honesty(s)
+    requires inv_only_dv_construct_signed_attestation_signature(s)
+    ensures inv_decided_value_of_consensus_instance_of_slot_k_is_for_slot_k(s) 
+    {
+        forall cid |
+            && cid in s.consensus_on_attestation_data.Keys
+            && s.consensus_on_attestation_data[cid].decided_value.isPresent()
+        {
+           lem_inv_decided_value_of_consensus_instance_of_slot_k_is_for_slot_k_helper(s, cid);
+        }        
+    }       
+
+    // 2 min    
+    // TODO: Simplify
+    lemma lem_inv_data_of_att_share_is_decided_value_att_consensus_decided(
+        s: DVState,
+        event: DV.Event,
+        s': DVState
+    )
+    requires NextEventPreCond(s, event)
+    requires NextEvent(s, event, s')  
+    requires event.HonestNodeTakingStep?
+    requires event.event.AttConsensusDecided?
+    requires inv_data_of_att_share_is_decided_value(s)
+    requires inv_decided_value_of_consensus_instance_of_slot_k_is_for_slot_k(s)
+    requires inv_attestation_shares_to_broadcast_is_a_subset_of_all_messages_sent(s)  
+    requires inv_quorum_constraints(s)
+    requires inv_unchanged_honesty(s)
+    requires same_honest_nodes_in_dv_and_ci(s)
+    requires inv_only_dv_construct_signed_attestation_signature(s)
+    requires inv_decided_value_of_consensus_instance_is_decided_by_quorum(s)    
+    requires inv_sent_validity_predicate_is_based_on_rcvd_att_duty_and_slashing_db(s)
+    requires inv_sent_validity_predicate_is_based_on_rcvd_att_duty_and_slashing_db_for_dv(s)          
+    requires |s.all_nodes| > 0
+    ensures inv_data_of_att_share_is_decided_value(s')   
+    {
+        match event 
+        {
+            case HonestNodeTakingStep(node, nodeEvent, nodeOutputs) =>
+                var process := s.honest_nodes_states[node];
+                var process' := s'.honest_nodes_states[node];
                 match nodeEvent
                 {
-                    case ServeAttstationDuty(att_duty) =>     
-                        lem_inv_rcvd_attn_shares_are_from_sent_messages_f_serve_attestation_duty(dvc, att_duty, dvc');                        
-                        
-                    case AttConsensusDecided(id, decided_attestation_data) => 
-                        lem_inv_rcvd_attn_shares_are_from_sent_messages_f_att_consensus_decided(dvc, id, decided_attestation_data, dvc');                        
-
-                    case ReceivedAttestationShare(attestation_share) =>    
-                        assert NetworkSpec.Next(dv.att_network, dv'.att_network, node, nodeOutputs.att_shares_sent, {attestation_share});
-                        assert multiset(addReceipientToMessages<AttestationShare>({attestation_share}, node)) <= dv.att_network.messagesInTransit;
-                        assert MessaageWithRecipient(message := attestation_share, receipient := node) in dv.att_network.messagesInTransit;        
-                        assert attestation_share in dv.att_network.allMessagesSent;
-                        assert attestation_share in dv'.att_network.allMessagesSent;
-                        
-                        lem_inv39_dv_next(dv, event, dv');
-                        assert dv.att_network.allMessagesSent <= dv'.att_network.allMessagesSent;
-                        
-                        lem_inv_rcvd_attn_shares_are_from_sent_messages_f_listen_for_attestation_shares(dvc, attestation_share, dvc');  
-
-                        assert dvc' == f_listen_for_attestation_shares(dvc, attestation_share).state;
-
-                        var k := (attestation_share.data, attestation_share.aggregation_bits);
-                        forall i, j | && i in dvc'.rcvd_attestation_shares.Keys 
-                                      && j in dvc'.rcvd_attestation_shares[i].Keys
-                        ensures dvc'.rcvd_attestation_shares[i][j] <= dv'.att_network.allMessagesSent;
+                    case AttConsensusDecided(id: Slot, decided_attestation_data) => 
+                        if  && process.current_attestation_duty.isPresent()
+                            && id == process.current_attestation_duty.safe_get().slot
+                            && id == decided_attestation_data.slot
                         {
-                            if ( || i != attestation_share.data.slot
-                                 || j != k
-                               )
-                            {             
-                                lem_inv_rcvd_attn_shares_are_from_sent_messages_f_listen_for_attestation_shares_domain(
-                                    dvc,
-                                    attestation_share,
-                                    dvc'
-                                );
-                                assert && i in dvc.rcvd_attestation_shares.Keys 
-                                       && j in dvc.rcvd_attestation_shares[i].Keys;
-                                assert dvc'.rcvd_attestation_shares[i][j] <= dvc.rcvd_attestation_shares[i][j];                                
-                                assert dvc.rcvd_attestation_shares[i][j] <= dv.att_network.allMessagesSent;
-                                lemmaSubsetOfSubset(
-                                    dvc'.rcvd_attestation_shares[i][j],
-                                    dvc.rcvd_attestation_shares[i][j],
-                                    dv.att_network.allMessagesSent
-                                );
-                                assert dv.att_network.allMessagesSent <= dv'.att_network.allMessagesSent;
-                                lemmaSubsetOfSubset(
-                                    dvc'.rcvd_attestation_shares[i][j],                                    
-                                    dv.att_network.allMessagesSent,
-                                    dv'.att_network.allMessagesSent
-                                );
-                                assert dvc'.rcvd_attestation_shares[i][j] <= dv'.att_network.allMessagesSent;
-                            }
-                            else
-                            {
-                                if  && i == attestation_share.data.slot
-                                    && j == k
-                                    && ( || i !in dvc.rcvd_attestation_shares.Keys
-                                         || j !in dvc.rcvd_attestation_shares[i].Keys
-                                       )                                       
-                                {
-                                    
-                                    assert dvc'.rcvd_attestation_shares[i][j] <= {attestation_share};
-                                    
-                                    
-                                    assert attestation_share in dv'.att_network.allMessagesSent;                                    
-                                    lemmaFromMemberToSingletonSet(attestation_share, dv'.att_network.allMessagesSent);
-                                    assert {attestation_share} <= dv'.att_network.allMessagesSent;
+                            var attestation_with_signature_share := f_calc_att_with_sign_share_from_decided_att_data(
+                                                                        process,
+                                                                        id,
+                                                                        decided_attestation_data
+                                                                    );       
+                            var messagesToBeSent := f_att_consensus_decided(process, id, decided_attestation_data).outputs.att_shares_sent;
 
-                                    lemmaSubsetOfSubset(
-                                            dvc'.rcvd_attestation_shares[i][j],
-                                            {attestation_share},
-                                            dv'.att_network.allMessagesSent
-                                        );
-                                    assert dvc'.rcvd_attestation_shares[i][j] <= dv'.att_network.allMessagesSent;                                     
-                                    
+                            assert messagesToBeSent ==  multicast(attestation_with_signature_share, process.peers);  
+                            assert s'.att_network.allMessagesSent == 
+                                        s.att_network.allMessagesSent + getMessagesFromMessagesWithRecipient(messagesToBeSent); 
+                            assert forall m | m in messagesToBeSent :: m.message == attestation_with_signature_share; 
+
+                            lemmaOnGetMessagesFromMessagesWithRecipientWhenAllMessagesAreTheSame(messagesToBeSent, attestation_with_signature_share);    
+                            assert getMessagesFromMessagesWithRecipient(messagesToBeSent) ==  {attestation_with_signature_share};
+                            assert s'.att_network.allMessagesSent == 
+                                        s.att_network.allMessagesSent + { attestation_with_signature_share }; 
+
+                            forall hn, att_share |
+                                    && hn in s'.honest_nodes_states.Keys 
+                                    && att_share in s'.att_network.allMessagesSent
+                                    && var fork_version := bn_get_fork_version(compute_start_slot_at_epoch(att_share.data.target.epoch));
+                                    && var attestation_signing_root := compute_attestation_signing_root(att_share.data, fork_version);
+                                    && verify_bls_siganture(attestation_signing_root, att_share.signature, hn)
+                            ensures s'.consensus_on_attestation_data[att_share.data.slot].decided_value.isPresent();
+                            ensures s'.consensus_on_attestation_data[att_share.data.slot].decided_value.safe_get() == att_share.data;     
+                            {
+                                // lem_inv_data_of_att_share_is_decided_value_att_consensus_decided_helper(s, event, s', hn, att_share);
+                                if att_share in s.att_network.allMessagesSent
+                                {
+                                    lem_inv_data_of_att_share_is_decided_value_att_consensus_decided_helper_1(s, event, s', hn, att_share);    
                                 }
                                 else
                                 {
-                                    assert  && i == attestation_share.data.slot
-                                            && j == k
-                                            && i in dvc.rcvd_attestation_shares.Keys 
-                                            && j in dvc.rcvd_attestation_shares[i].Keys;
+                                    assert att_share == attestation_with_signature_share;
+                                    lemmaImaptotalElementInDomainIsInKeys(s.consensus_on_attestation_data, id);
+                                    assert id in s.consensus_on_attestation_data.Keys ;
+                                    lem_inv_data_of_att_share_is_decided_value_att_consensus_decided_helper_2(s, event, s');
 
+                                    assert s'.consensus_on_attestation_data[id].decided_value.safe_get() == decided_attestation_data; 
+                                    assert s'.consensus_on_attestation_data[id].decided_value.safe_get() == att_share.data; 
+                                    lem_inv_decided_value_of_consensus_instance_of_slot_k_is_for_slot_k(s, event, s');   
                                     
-                                    assert dvc'.rcvd_attestation_shares[i][j] 
-                                                <= dvc.rcvd_attestation_shares[i][j] + {attestation_share}; 
+                                    assert att_share.data.slot == id;
+                                    assert s'.consensus_on_attestation_data[att_share.data.slot].decided_value.isPresent();                             
+                                    assert s'.consensus_on_attestation_data[att_share.data.slot].decided_value.safe_get() == att_share.data; 
+                                } 
+                            }           
 
-                                    assert dvc.rcvd_attestation_shares[i][j] 
-                                                <= dv.att_network.allMessagesSent;                                                
-                                    assert dv.att_network.allMessagesSent <= dv'.att_network.allMessagesSent;      
-                                    lemmaSubsetOfSubset(
-                                        dvc.rcvd_attestation_shares[i][j],
-                                        dv.att_network.allMessagesSent,
-                                        dv'.att_network.allMessagesSent);                                    
-                                    assert dvc.rcvd_attestation_shares[i][j] 
-                                                <= dv'.att_network.allMessagesSent;
-
-                                    assert attestation_share in dv'.att_network.allMessagesSent;                                    
-                                    lemmaFromMemberToSingletonSet(attestation_share, dv'.att_network.allMessagesSent);
-                                    assert {attestation_share} <= dv'.att_network.allMessagesSent;
-
-                                    lemmaUnionOfSubsets(dvc.rcvd_attestation_shares[i][j], {attestation_share}, dv'.att_network.allMessagesSent);                                    
-                                    assert dvc.rcvd_attestation_shares[i][j] + {attestation_share}
-                                                <= dv'.att_network.allMessagesSent;
-
-                                    lemmaSubsetOfSubset(
-                                        dvc'.rcvd_attestation_shares[i][j],
-                                        dvc.rcvd_attestation_shares[i][j] + {attestation_share},
-                                        dv'.att_network.allMessagesSent);
-                                    
-                                    assert dvc'.rcvd_attestation_shares[i][j] <= dv'.att_network.allMessagesSent;                                                                         
-                                }
-                            }
+                            assert inv_data_of_att_share_is_decided_value(s');
                         }
-                        assert inv_rcvd_attn_shares_are_from_sent_messages(dv');
+                        else 
+                        {
+                            forall hn, att_share |
+                                    && hn in s'.honest_nodes_states.Keys 
+                                    && att_share in s'.att_network.allMessagesSent
+                                    && var fork_version := bn_get_fork_version(compute_start_slot_at_epoch(att_share.data.target.epoch));
+                                    && var attestation_signing_root := compute_attestation_signing_root(att_share.data, fork_version);
+                                    && verify_bls_siganture(attestation_signing_root, att_share.signature, hn)
+                            ensures s'.consensus_on_attestation_data[att_share.data.slot].decided_value.isPresent();
+                            ensures s'.consensus_on_attestation_data[att_share.data.slot].decided_value.safe_get() == att_share.data;     
+                            {
+                                assert att_share in s.att_network.allMessagesSent;
+                                lem_inv_data_of_att_share_is_decided_value_att_consensus_decided_helper_1(s, event, s', hn, att_share);
+                            } 
 
-                    case ImportedNewBlock(block) => 
-                        var dvc_mod := f_add_block_to_bn(dvc, block);
-                        lem_inv_rcvd_attn_shares_are_from_sent_messages_f_add_block_to_bn(dvc, block, dvc_mod);
-                        lem_inv_rcvd_attn_shares_are_from_sent_messages_f_listen_for_new_imported_blocks(dvc_mod, block, dvc');                                                
-                                                
-                    case ResendAttestationShares =>                         
-                        lem_inv_rcvd_attn_shares_are_from_sent_messages_f_resend_attestation_share(dvc, dvc');
-
-                    case NoEvent => 
-                        
+                            assert inv_data_of_att_share_is_decided_value(s');
+                        }
                 }
+        }
+    }
 
-            case AdeversaryTakingStep(node, new_attestation_share_sent, messagesReceivedByTheNode) =>
-                
-        }        
-    }  
-
-    lemma lem_inv_available_latest_attestation_duty_is_from_dv_seq_of_att_duties_new_body_dv_next(
-        dv: DVState,
+    lemma lem_inv_data_of_att_share_is_decided_value_att_adversary(
+        s: DVState,
         event: DV.Event,
-        dv': DVState
+        s': DVState
+    )
+    requires NextEventPreCond(s, event)
+    requires NextEvent(s, event, s')  
+    requires event.AdeversaryTakingStep?
+    requires inv_data_of_att_share_is_decided_value(s)
+    requires inv_decided_value_of_consensus_instance_of_slot_k_is_for_slot_k(s)
+    requires inv_attestation_shares_to_broadcast_is_a_subset_of_all_messages_sent(s)  
+    requires inv_quorum_constraints(s)
+    requires same_honest_nodes_in_dv_and_ci(s)
+    requires inv_only_dv_construct_signed_attestation_signature(s)
+    requires |s.all_nodes| > 0
+    ensures inv_data_of_att_share_is_decided_value(s') 
+    {
+        var new_attestation_shares_sent := s'.att_network.allMessagesSent - s.att_network.allMessagesSent;
+
+        forall hn, att_share |
+                && hn in s'.honest_nodes_states.Keys 
+                && att_share in s'.att_network.allMessagesSent
+                && var fork_version := bn_get_fork_version(compute_start_slot_at_epoch(att_share.data.target.epoch));
+                && var attestation_signing_root := compute_attestation_signing_root(att_share.data, fork_version);
+                && verify_bls_siganture(attestation_signing_root, att_share.signature, hn)
+        ensures s'.consensus_on_attestation_data[att_share.data.slot].decided_value.isPresent();
+        ensures s'.consensus_on_attestation_data[att_share.data.slot].decided_value.safe_get() == att_share.data;                          
+        {
+            var fork_version := bn_get_fork_version(compute_start_slot_at_epoch(att_share.data.target.epoch));
+            var attestation_signing_root := compute_attestation_signing_root(att_share.data, fork_version);        
+
+            if att_share in s.att_network.allMessagesSent
+            {
+                assert s.consensus_on_attestation_data[att_share.data.slot].decided_value.isPresent();
+                assert s.consensus_on_attestation_data[att_share.data.slot].decided_value.safe_get() == att_share.data;   
+            }
+            else
+            {
+                forall signer | verify_bls_siganture(attestation_signing_root, att_share.signature, signer)
+                ensures signer in s.adversary.nodes;
+                ensures signer !in  s.honest_nodes_states.Keys; 
+                {
+
+                    assert signer in s.adversary.nodes; 
+                    lemmaEmptyIntersectionImpliesDisjointness(s.adversary.nodes, s.honest_nodes_states.Keys);
+                    assert s.adversary.nodes !! s.honest_nodes_states.Keys;
+                    assert signer !in  s.honest_nodes_states.Keys;
+                }              
+                assert false;          
+            }
+        }
+    
+        assert inv_data_of_att_share_is_decided_value(s');
+    }      
+
+    lemma lem_inv_data_of_att_share_is_decided_value_helper2<M>(
+        allMessagesSent': set<M>,
+        allMessagesSent: set<M>,
+        messagesToBeSent: set<MessaageWithRecipient<M>>
+    )
+    requires allMessagesSent' == allMessagesSent + 
+                                getMessagesFromMessagesWithRecipient(messagesToBeSent);
+    requires messagesToBeSent == {}
+    ensures allMessagesSent' == allMessagesSent
+    { }
+
+       
+
+    lemma lem_inv_sent_validity_predicate_is_based_on_rcvd_att_duty_and_slashing_db_for_dvc_updateConsensusInstanceValidityCheckHelper(
+        m: map<Slot, AttestationConsensusValidityCheckState>,
+        new_attestation_slashing_db: set<SlashingDBAttestation>,
+        m': map<Slot, AttestationConsensusValidityCheckState>
     )    
-    requires NextEvent.requires(dv, event, dv')  
-    requires NextEvent(dv, event, dv')  
-    requires inv_latest_attestation_duty_is_from_dv_seq_of_att_duties(dv)
-    ensures inv_latest_attestation_duty_is_from_dv_seq_of_att_duties(dv')
-    {        
+    requires m' == updateConsensusInstanceValidityCheckHelper(m, new_attestation_slashing_db)
+    requires forall k | k in m :: inv_sent_validity_predicate_is_based_on_rcvd_att_duty_and_slashing_db_for_dvc_single_dvc_2_body_body(k, m[k].attestation_duty, m[k].validityPredicate)
+    ensures forall k | k in m' :: inv_sent_validity_predicate_is_based_on_rcvd_att_duty_and_slashing_db_for_dvc_single_dvc_2_body_body(k, m'[k].attestation_duty, m'[k].validityPredicate)    
+    {
+        forall k | k in  m 
+        ensures k in m'
+        {
+            lemmaMapKeysHasOneEntryInItems(m, k);
+            assert k in m';
+        }
+
+        assert m.Keys == m'.Keys;
+
+        forall k | k in m' 
+        ensures inv_sent_validity_predicate_is_based_on_rcvd_att_duty_and_slashing_db_body(k, m'[k].attestation_duty, new_attestation_slashing_db, m'[k].validityPredicate); 
+        {
+            assert m'[k] == m[k].(
+                    validityPredicate := (ad: AttestationData) => consensus_is_valid_attestation_data(new_attestation_slashing_db, ad, m[k].attestation_duty)
+            );
+            assert  inv_sent_validity_predicate_is_based_on_rcvd_att_duty_and_slashing_db_body(k, m'[k].attestation_duty, new_attestation_slashing_db, m'[k].validityPredicate);        
+        }
+    }
+
+    
+    lemma lem_inv_db_of_validity_predicate_contains_all_previous_decided_values_f_check_for_next_duty_updateConsensusInstanceValidityCheck(
+        s: ConsensusEngineState,
+        new_attestation_slashing_db: set<SlashingDBAttestation>,
+        s': ConsensusEngineState
+    )    
+    requires s' == updateConsensusInstanceValidityCheck(s, new_attestation_slashing_db)
+    ensures s'.active_attestation_consensus_instances.Keys == s.active_attestation_consensus_instances.Keys
+    ensures s'.att_slashing_db_hist.Keys == s.att_slashing_db_hist.Keys + s'.active_attestation_consensus_instances.Keys;
+    {
+        lem_updateConsensusInstanceValidityCheckHelper(s.active_attestation_consensus_instances, new_attestation_slashing_db, s'.active_attestation_consensus_instances);
+
+        assert s'.att_slashing_db_hist.Keys == s.att_slashing_db_hist.Keys + s'.active_attestation_consensus_instances.Keys;
+
+        assert forall slot, vp: AttestationData -> bool |
+                    && slot in s.att_slashing_db_hist.Keys 
+                    && vp in s.att_slashing_db_hist[slot].Keys
+                    ::
+                    && s.att_slashing_db_hist.Keys <= s'.att_slashing_db_hist.Keys
+                    && s.att_slashing_db_hist[slot].Keys <= s'.att_slashing_db_hist[slot].Keys
+                    && s.att_slashing_db_hist[slot][vp] <= s'.att_slashing_db_hist[slot][vp]
+        ;
+
+        assert forall slot |
+                    && slot in s'.active_attestation_consensus_instances.Keys 
+                    && slot in s.att_slashing_db_hist.Keys
+                    && var vp := s'.active_attestation_consensus_instances[slot].validityPredicate;
+                    && vp in s.att_slashing_db_hist[slot].Keys
+                    ::
+                    var vp := s'.active_attestation_consensus_instances[slot].validityPredicate;
+                    s.att_slashing_db_hist[slot][vp] + {new_attestation_slashing_db} == s'.att_slashing_db_hist[slot][vp];      
+
+        assert forall slot, vp: AttestationData -> bool |
+                    && slot in s'.att_slashing_db_hist.Keys 
+                    && slot !in s.att_slashing_db_hist.Keys 
+                    && vp in s'.att_slashing_db_hist[slot].Keys
+                    ::
+                    && vp == s'.active_attestation_consensus_instances[slot].validityPredicate
+        ;      
+
+        assert forall slot, vp: AttestationData -> bool |
+                    && slot in s.att_slashing_db_hist.Keys 
+                    && vp in s'.att_slashing_db_hist[slot].Keys
+                    && vp !in s.att_slashing_db_hist[slot].Keys
+                    ::
+                    && s'.att_slashing_db_hist[slot][vp] == {new_attestation_slashing_db}
+        ;     
+                   
+    }   
+
+    lemma lem_inv_db_of_validity_predicate_contains_all_previous_decided_values_f_check_for_next_duty_updateConsensusInstanceValidityCheck2(
+        s: ConsensusEngineState,
+        new_attestation_slashing_db: set<SlashingDBAttestation>,
+        s': ConsensusEngineState,
+        slot: nat,
+        vp: AttestationData -> bool 
+    )    
+    requires s' == updateConsensusInstanceValidityCheck(s, new_attestation_slashing_db)
+    requires 
+                    && slot in s'.active_attestation_consensus_instances.Keys 
+                    && slot in s.att_slashing_db_hist.Keys
+                    && vp == s'.active_attestation_consensus_instances[slot].validityPredicate
+                    && vp in s.att_slashing_db_hist[slot].Keys  
+    ensures s.att_slashing_db_hist[slot][vp] + {new_attestation_slashing_db} == s'.att_slashing_db_hist[slot][vp];      
+    {
+        lem_updateConsensusInstanceValidityCheckHelper(s.active_attestation_consensus_instances, new_attestation_slashing_db, s'.active_attestation_consensus_instances);
+
+        assert s'.att_slashing_db_hist.Keys == s.att_slashing_db_hist.Keys + s'.active_attestation_consensus_instances.Keys;                   
+    }   
+
+    lemma lem_inv_db_of_validity_predicate_contains_all_previous_decided_values_f_check_for_next_duty_updateConsensusInstanceValidityCheck3(
+        s: ConsensusEngineState,
+        new_attestation_slashing_db: set<SlashingDBAttestation>,
+        s': ConsensusEngineState,
+        slot: nat,
+        vp: AttestationData -> bool 
+    )    
+    requires s' == updateConsensusInstanceValidityCheck(s, new_attestation_slashing_db)
+    requires 
+                    && slot in s'.active_attestation_consensus_instances.Keys 
+                    && slot in s.att_slashing_db_hist.Keys
+                    && vp != s'.active_attestation_consensus_instances[slot].validityPredicate
+                    && vp in s.att_slashing_db_hist[slot].Keys  
+    ensures s.att_slashing_db_hist[slot][vp] == s'.att_slashing_db_hist[slot][vp];      
+    {
+        lem_updateConsensusInstanceValidityCheckHelper(s.active_attestation_consensus_instances, new_attestation_slashing_db, s'.active_attestation_consensus_instances);
+
+        assert s'.att_slashing_db_hist.Keys == s.att_slashing_db_hist.Keys + s'.active_attestation_consensus_instances.Keys;                   
+    }      
+
+    lemma lem_inv_db_of_validity_predicate_contains_all_previous_decided_values_f_check_for_next_duty_updateConsensusInstanceValidityCheck4(
+        s: ConsensusEngineState,
+        new_attestation_slashing_db: set<SlashingDBAttestation>,
+        s': ConsensusEngineState,
+        slot: nat,
+        vp: AttestationData -> bool 
+    )    
+    requires s' == updateConsensusInstanceValidityCheck(s, new_attestation_slashing_db)
+    requires 
+                    && slot !in s'.active_attestation_consensus_instances.Keys 
+                    && slot in s.att_slashing_db_hist.Keys
+                    && vp in s.att_slashing_db_hist[slot].Keys  
+    ensures s.att_slashing_db_hist[slot][vp] == s'.att_slashing_db_hist[slot][vp];      
+    {
+        lem_updateConsensusInstanceValidityCheckHelper(s.active_attestation_consensus_instances, new_attestation_slashing_db, s'.active_attestation_consensus_instances);
+
+        assert s'.att_slashing_db_hist.Keys == s.att_slashing_db_hist.Keys + s'.active_attestation_consensus_instances.Keys;                   
+    }   
+
+    lemma lem_inv_db_of_validity_predicate_contains_all_previous_decided_values_f_check_for_next_duty_updateConsensusInstanceValidityCheck5(
+        s: ConsensusEngineState,
+        new_attestation_slashing_db: set<SlashingDBAttestation>,
+        s': ConsensusEngineState,
+        slot: nat    
+    )    
+    requires s' == updateConsensusInstanceValidityCheck(s, new_attestation_slashing_db)
+    requires slot in s.att_slashing_db_hist.Keys
+    ensures slot in s'.att_slashing_db_hist.Keys
+    ensures s.att_slashing_db_hist[slot].Keys <= s'.att_slashing_db_hist[slot].Keys;      
+    {
+        lem_updateConsensusInstanceValidityCheckHelper(s.active_attestation_consensus_instances, new_attestation_slashing_db, s'.active_attestation_consensus_instances);
+
+        assert s'.att_slashing_db_hist.Keys == s.att_slashing_db_hist.Keys + s'.active_attestation_consensus_instances.Keys;                   
+    }    
+
+    lemma lem_inv_sent_validity_predicate_is_based_on_rcvd_att_duty_and_slashing_db_for_dvc_single_dvc_2_f_terminate_current_attestation_duty(
+        process: DVCState,
+        process': DVCState
+    )
+    requires f_terminate_current_attestation_duty.requires(process)
+    requires process' == f_terminate_current_attestation_duty(process)
+    requires inv_sent_validity_predicate_is_based_on_rcvd_att_duty_and_slashing_db_for_dvc_single_dvc_2(process)
+    ensures inv_sent_validity_predicate_is_based_on_rcvd_att_duty_and_slashing_db_for_dvc_single_dvc_2(process')
+    { }       
+
+    // TODO: new proof
+    lemma lem_inv_sent_validity_predicate_is_based_on_rcvd_att_duty_and_slashing_db_for_dvc_f_check_for_next_duty_helper(
+        process: DVCState,
+        attestation_duty: AttestationDuty,
+        s': DVCState
+    )
+    requires f_check_for_next_duty.requires(process, attestation_duty)
+    requires s' == f_check_for_next_duty(process, attestation_duty).state   
+    requires inv_sent_validity_predicate_is_based_on_rcvd_att_duty_and_slashing_db_for_dvc_single_dvc_2(process) 
+    // ensures  inv_sent_validity_predicate_is_based_on_rcvd_att_duty_and_slashing_db_for_dvc_single_dvc_2(s')
+    {
+        var attestation_slashing_db := process.attestation_slashing_db;
+
+        var acvc := AttestationConsensusValidityCheckState(
+            attestation_duty := attestation_duty,
+            validityPredicate := (ad: AttestationData) => consensus_is_valid_attestation_data(attestation_slashing_db, ad, attestation_duty)
+        );     
+
+        // assert s'.attestation_consensus_engine_state.active_attestation_consensus_instances == process.attestation_consensus_engine_state.active_attestation_consensus_instances[attestation_duty.slot := acvc];
+
+
+        forall cid | cid in s'.attestation_consensus_engine_state.active_attestation_consensus_instances  
+            // ensures inv_sent_validity_predicate_is_based_on_rcvd_att_duty_and_slashing_db_for_dvc_single_dvc_2_body(s', cid); 
+        {
+            if cid != attestation_duty.slot 
+            {
+                assert cid in process.attestation_consensus_engine_state.active_attestation_consensus_instances;
+                // assert inv_sent_validity_predicate_is_based_on_rcvd_att_duty_and_slashing_db_for_dvc_single_dvc_2_body(s', cid); 
+            }
+            else 
+            {
+                assert inv_sent_validity_predicate_is_based_on_rcvd_att_duty_and_slashing_db_body(
+                    cid,
+                    attestation_duty,
+                    attestation_slashing_db,
+                    acvc.validityPredicate
+                );
+                assert inv_sent_validity_predicate_is_based_on_rcvd_att_duty_and_slashing_db_for_dvc_single_dvc_2_body(s', cid); 
+            }
+        }   
+    }
+
+    lemma lem_inv_sent_validity_predicate_is_based_on_rcvd_att_duty_and_slashing_db_for_dvc_f_start_next_duty(
+        process: DVCState,
+        attestation_duty: AttestationDuty,
+        process': DVCState
+    )
+    requires f_check_for_next_duty.requires(process, attestation_duty)
+    requires process' == f_start_next_duty(process, attestation_duty).state   
+    requires inv_sent_validity_predicate_is_based_on_rcvd_att_duty_and_slashing_db_for_dvc_single_dvc_2(process) 
+    ensures inv_sent_validity_predicate_is_based_on_rcvd_att_duty_and_slashing_db_for_dvc_single_dvc_2(process')
+    {
+        var new_process := f_new_process_after_starting_new_att_duty(process, attestation_duty);
+
+        assert { attestation_duty.slot } ==
+                     new_process.attestation_consensus_engine_state.active_attestation_consensus_instances.Keys - 
+                            process.attestation_consensus_engine_state.active_attestation_consensus_instances.Keys;
+
+        forall cid | cid in new_process.attestation_consensus_engine_state.active_attestation_consensus_instances
+        ensures inv_sent_validity_predicate_is_based_on_rcvd_att_duty_and_slashing_db_for_dvc_single_dvc_2_body(new_process, cid) 
+        { 
+            if cid in process.attestation_consensus_engine_state.active_attestation_consensus_instances
+            {
+                assert inv_sent_validity_predicate_is_based_on_rcvd_att_duty_and_slashing_db_for_dvc_single_dvc_2_body(new_process, cid);
+            }
+            else
+            {
+                assert cid == attestation_duty.slot;
+                
+                var acvc := AttestationConsensusValidityCheckState(
+                    attestation_duty := attestation_duty,
+                    validityPredicate := (ad: AttestationData) => consensus_is_valid_attestation_data(process.attestation_slashing_db, ad, attestation_duty)
+                );
+
+                assert acvc == process'.attestation_consensus_engine_state.active_attestation_consensus_instances[cid];
+                assert inv_sent_validity_predicate_is_based_on_rcvd_att_duty_and_slashing_db_body(cid, attestation_duty, process.attestation_slashing_db, acvc.validityPredicate);    
+                assert inv_sent_validity_predicate_is_based_on_rcvd_att_duty_and_slashing_db_for_dvc_single_dvc_2_body_body(cid, attestation_duty, acvc.validityPredicate);
+                assert inv_sent_validity_predicate_is_based_on_rcvd_att_duty_and_slashing_db_for_dvc_single_dvc_2_body(new_process, cid);
+            }
+        }
+    }
+    
+    lemma lem_inv_sent_validity_predicate_is_based_on_rcvd_att_duty_and_slashing_db_for_dvc_single_dvc_2_f_check_for_next_duty(
+        process: DVCState,
+        attestation_duty: AttestationDuty,
+        process': DVCState
+    )
+    requires f_check_for_next_duty.requires(process, attestation_duty)
+    requires process' == f_check_for_next_duty(process, attestation_duty).state   
+    requires inv_sent_validity_predicate_is_based_on_rcvd_att_duty_and_slashing_db_for_dvc_single_dvc_2(process) 
+    ensures inv_sent_validity_predicate_is_based_on_rcvd_att_duty_and_slashing_db_for_dvc_single_dvc_2(process'); 
+    {
+        if pred_decision_of_att_duty_was_known(process, attestation_duty)
+        {                
+            var new_process := f_new_process_after_updateConsensusInstanceValidityCheck(process, attestation_duty);
+
+            lem_inv_sent_validity_predicate_is_based_on_rcvd_att_duty_and_slashing_db_for_dvc_updateConsensusInstanceValidityCheckHelper(
+                    process.attestation_consensus_engine_state.active_attestation_consensus_instances,
+                    new_process.attestation_slashing_db,
+                    new_process.attestation_consensus_engine_state.active_attestation_consensus_instances
+            );
+        }
+        else 
+        {
+            lem_inv_sent_validity_predicate_is_based_on_rcvd_att_duty_and_slashing_db_for_dvc_f_start_next_duty(
+                process,
+                attestation_duty,
+                process'
+            );                
+        }    
+    }        
+
+    lemma lem_inv_sent_validity_predicate_is_based_on_rcvd_att_duty_and_slashing_db_for_dvc_single_dvc_2_f_serve_attestation_duty(
+        process: DVCState,
+        attestation_duty: AttestationDuty,
+        process': DVCState
+    )
+    requires f_serve_attestation_duty.requires(process, attestation_duty)
+    requires process' == f_serve_attestation_duty(process, attestation_duty).state  
+    requires inv_sent_validity_predicate_is_based_on_rcvd_att_duty_and_slashing_db_for_dvc_single_dvc_2(process) 
+    ensures inv_sent_validity_predicate_is_based_on_rcvd_att_duty_and_slashing_db_for_dvc_single_dvc_2(process'); 
+    {
+        var process_rcvd_duty := 
+                process.(all_rcvd_duties := process.all_rcvd_duties + {attestation_duty});
+        var process_after_stopping_active_consensus_instance := f_terminate_current_attestation_duty(process_rcvd_duty);
+        lem_inv_sent_validity_predicate_is_based_on_rcvd_att_duty_and_slashing_db_for_dvc_single_dvc_2_f_terminate_current_attestation_duty(
+            process_rcvd_duty,
+            process_after_stopping_active_consensus_instance
+        );
+        lem_inv_sent_validity_predicate_is_based_on_rcvd_att_duty_and_slashing_db_for_dvc_single_dvc_2_f_check_for_next_duty(
+            process_after_stopping_active_consensus_instance,
+            attestation_duty,
+            process'
+        );        
+    }        
+
+    lemma lem_inv_sent_validity_predicate_is_based_on_rcvd_att_duty_and_slashing_db_for_dvc_single_dvc_2_f_att_consensus_decided(
+        process: DVCState,
+        id: Slot,
+        decided_attestation_data: AttestationData,        
+        s': DVCState
+    )
+    requires f_att_consensus_decided.requires(process, id, decided_attestation_data)
+    requires s' == f_att_consensus_decided(process, id, decided_attestation_data).state
+    requires inv_sent_validity_predicate_is_based_on_rcvd_att_duty_and_slashing_db_for_dvc_single_dvc_2(process) 
+    ensures inv_sent_validity_predicate_is_based_on_rcvd_att_duty_and_slashing_db_for_dvc_single_dvc_2(s'); 
+    {
+        if pred_att_duty_was_already_decided(process, id) 
+        {
+            var s_mod := f_update_process_after_att_duty_decided(
+                            process,
+                            id,
+                            decided_attestation_data);
+
+            lem_inv_sent_validity_predicate_is_based_on_rcvd_att_duty_and_slashing_db_for_dvc_updateConsensusInstanceValidityCheckHelper(
+                    process.attestation_consensus_engine_state.active_attestation_consensus_instances,
+                    s_mod.attestation_slashing_db,
+                    s_mod.attestation_consensus_engine_state.active_attestation_consensus_instances
+            );            
+        }            
+    }     
+
+    lemma lem_inv_sent_validity_predicate_is_based_on_rcvd_att_duty_and_slashing_db_f_listen_for_new_imported_blocks(
+        process: DVCState,
+        block: BeaconBlock,
+        s': DVCState
+    )
+    requires f_listen_for_new_imported_blocks.requires(process, block)
+    requires s' == f_listen_for_new_imported_blocks(process, block).state
+    requires inv_sent_validity_predicate_is_based_on_rcvd_att_duty_and_slashing_db_for_dvc_single_dvc_2(process) 
+    ensures inv_sent_validity_predicate_is_based_on_rcvd_att_duty_and_slashing_db_for_dvc_single_dvc_2(s');     
+    {
+        var new_consensus_instances_already_decided := f_listen_for_new_imported_blocks_helper_1(process, block);
+
+        var att_consensus_instances_already_decided := process.future_att_consensus_instances_already_decided + new_consensus_instances_already_decided;
+
+        var process := f_stopConsensusInstances_after_receiving_new_imported_blocks(
+                                process,
+                                block
+                            );
+
+        if pred_listen_for_new_imported_blocks_checker(process, att_consensus_instances_already_decided)
+        {
+            var s_mod := f_updateConsensusInstanceValidityCheck_in_listen_for_new_imported_blocks(
+                                    process,
+                                    att_consensus_instances_already_decided
+                                );
+
+            lem_inv_sent_validity_predicate_is_based_on_rcvd_att_duty_and_slashing_db_for_dvc_updateConsensusInstanceValidityCheckHelper(
+                    process.attestation_consensus_engine_state.active_attestation_consensus_instances,
+                    s_mod.attestation_slashing_db,
+                    s_mod.attestation_consensus_engine_state.active_attestation_consensus_instances
+            );            
+        }
+    }      
+
+    lemma lem_inv_sent_validity_predicate_is_based_on_rcvd_att_duty_and_slashing_db_for_dv(
+        s: DVState,
+        event: DV.Event,
+        s': DVState
+    )   
+    requires NextEventPreCond(s, event)
+    requires NextEvent(s, event, s')    
+    requires inv_quorum_constraints(s)
+    requires inv_unchanged_honesty(s)
+    requires inv_only_dv_construct_signed_attestation_signature(s)      
+    requires inv_sent_validity_predicate_is_based_on_rcvd_att_duty_and_slashing_db_for_dv(s)  
+    ensures inv_sent_validity_predicate_is_based_on_rcvd_att_duty_and_slashing_db_for_dv(s')    
+    {
         match event 
         {
             case HonestNodeTakingStep(node, nodeEvent, nodeOutputs) =>
-                var dvc := dv.honest_nodes_states[node];
-                var dvc' := dv'.honest_nodes_states[node];   
-                
+                var s_node := s.honest_nodes_states[node];
+                var s'_node := s'.honest_nodes_states[node];
                 match nodeEvent
                 {
-                    case ServeAttstationDuty(attestation_duty) =>                           
-                        
+                    case ServeAttstationDuty(attestation_duty) => 
+                        forall n | n in s'.honest_nodes_states
+                        ensures inv_sent_validity_predicate_is_based_on_rcvd_att_duty_and_slashing_db_for_dvc_single_dvc_2(s'.honest_nodes_states[n]); 
+                        {
+                            if n == node
+                            {
+                                lem_inv_sent_validity_predicate_is_based_on_rcvd_att_duty_and_slashing_db_for_dvc_single_dvc_2_f_serve_attestation_duty(s_node, attestation_duty, s'_node);
+                                assert inv_sent_validity_predicate_is_based_on_rcvd_att_duty_and_slashing_db_for_dvc_single_dvc_2(s'_node); 
+                            }
+                        }
+                        assert inv_sent_validity_predicate_is_based_on_rcvd_att_duty_and_slashing_db_for_dv(s');                        
+                  
                     case AttConsensusDecided(id, decided_attestation_data) => 
-                        
-                    case ReceivedAttestationShare(attestation_share) =>                         
-                       
-                    case ImportedNewBlock(block) => 
-                
-                    case ResendAttestationShares =>                                                                      
+                        forall n | n in s'.honest_nodes_states
+                        ensures inv_sent_validity_predicate_is_based_on_rcvd_att_duty_and_slashing_db_for_dvc_single_dvc_2(s'.honest_nodes_states[n]); 
+                        {
+                            if n == node
+                            {
+                                lem_inv_sent_validity_predicate_is_based_on_rcvd_att_duty_and_slashing_db_for_dvc_single_dvc_2_f_att_consensus_decided(s_node, id, decided_attestation_data, s'_node);
+                                assert inv_sent_validity_predicate_is_based_on_rcvd_att_duty_and_slashing_db_for_dvc_single_dvc_2(s'_node); 
+                            }
+                        }
+                        assert inv_sent_validity_predicate_is_based_on_rcvd_att_duty_and_slashing_db_for_dv(s');                       
+              
+                    case ReceivedAttestationShare(attestation_share) => 
+                        forall n | n in s'.honest_nodes_states
+                        ensures s'.honest_nodes_states[n].attestation_consensus_engine_state == s.honest_nodes_states[n].attestation_consensus_engine_state
+                        {
+                            if n == node
+                            {
+                                lem_f_listen_for_attestation_shares_unchanged_dvc_vars(s_node, attestation_share, s'_node);
+                            }
+                        }
+                        assert inv_sent_validity_predicate_is_based_on_rcvd_att_duty_and_slashing_db_for_dv(s');     
 
+                    case ImportedNewBlock(block) => 
+                        forall n | n in s'.honest_nodes_states
+                        ensures inv_sent_validity_predicate_is_based_on_rcvd_att_duty_and_slashing_db_for_dvc_single_dvc_2(s'.honest_nodes_states[n]); 
+                        {
+                            if n == node
+                            {
+                                var s_node := f_add_block_to_bn(s_node, nodeEvent.block);
+                                lem_inv_sent_validity_predicate_is_based_on_rcvd_att_duty_and_slashing_db_f_listen_for_new_imported_blocks(s_node, block, s'_node);
+                                assert inv_sent_validity_predicate_is_based_on_rcvd_att_duty_and_slashing_db_for_dvc_single_dvc_2(s'_node); 
+                            }
+                        }
+                        assert inv_sent_validity_predicate_is_based_on_rcvd_att_duty_and_slashing_db_for_dv(s');                        
+               
+                    case ResendAttestationShares => 
+                        assert inv_sent_validity_predicate_is_based_on_rcvd_att_duty_and_slashing_db_for_dv(s');
+                   
                     case NoEvent => 
-                        
-                }
-                
+                        assert inv_sent_validity_predicate_is_based_on_rcvd_att_duty_and_slashing_db_for_dv(s');
+                }            
+
+
             case AdeversaryTakingStep(node, new_attestation_share_sent, messagesReceivedByTheNode) =>
-                
-        }   
-    }      
-}   
-        
+                assert inv_sent_validity_predicate_is_based_on_rcvd_att_duty_and_slashing_db_for_dv(s');
+        }        
+    } 
+
+    lemma lem_f_listen_for_new_imported_blocks_helper_1(
+        dv: DVState,
+        process: DVCState,
+        block: BeaconBlock,
+        new_consensus_instances_already_decided: map<Slot, AttestationData>
+    )
+    requires f_listen_for_new_imported_blocks_helper_1.requires(process, block)
+    requires new_consensus_instances_already_decided == f_listen_for_new_imported_blocks_helper_1(process, block)
+    requires inv_exists_honest_dvc_that_sent_att_share_for_submitted_att(dv)
+    requires inv_data_of_att_share_is_decided_value(dv)
+    requires pred_axiom_is_my_attestation_2(dv, process, block)
+    ensures forall slot | 
+                slot in new_consensus_instances_already_decided
+                :: 
+                && dv.consensus_on_attestation_data[slot].decided_value.isPresent()
+                && dv.consensus_on_attestation_data[slot].decided_value.safe_get() == new_consensus_instances_already_decided[slot]
+                ;  
+    {
+        forall slot | slot in new_consensus_instances_already_decided
+        ensures 
+            && dv.consensus_on_attestation_data[slot].decided_value.isPresent()
+            && dv.consensus_on_attestation_data[slot].decided_value.safe_get() == new_consensus_instances_already_decided[slot]
+            ;         
+        {
+
+            var valIndex := bn_get_validator_index(process.bn, block.body.state_root, process.dv_pubkey);
+
+
+            var a :| 
+                && a in block.body.attestations
+                && DVC_Spec_NonInstr.isMyAttestation(a, process.bn, block, valIndex)
+                && a.data == new_consensus_instances_already_decided[slot]
+            ;
+
+            var a' :|
+                && a' in dv.all_attestations_created
+                && a'.data == a.data 
+                && is_valid_attestation(a', dv.dv_pubkey);    
+
+            var hn', att_share: AttestationShare :| inv_exists_honest_dvc_that_sent_att_share_for_submitted_att_body(dv, hn', att_share, a');
+
+            assert
+            && dv.consensus_on_attestation_data[att_share.data.slot].decided_value.isPresent()
+            && dv.consensus_on_attestation_data[att_share.data.slot].decided_value.safe_get() == att_share.data;
+
+            assert
+            && dv.consensus_on_attestation_data[slot].decided_value.isPresent()
+            && dv.consensus_on_attestation_data[slot].decided_value.safe_get() == new_consensus_instances_already_decided[slot]
+            ;              
+        }
+    }  
+
+    lemma lem_inv_sequence_attestation_duties_to_be_served_orderd(
+        s: DVState,
+        event: DV.Event,
+        s': DVState
+    )
+    requires NextEventPreCond(s, event)
+    requires NextEvent(s, event, s')  
+    requires is_sequence_attestation_duties_to_be_served_orderd(s)
+    ensures is_sequence_attestation_duties_to_be_served_orderd(s')
+    {
+        match event 
+        {
+            case HonestNodeTakingStep(node, nodeEvent, nodeOutputs) =>
+                assert s'.sequence_attestation_duties_to_be_served == s.sequence_attestation_duties_to_be_served;
+            
+            case AdeversaryTakingStep(node, new_attestation_share_sent, messagesReceivedByTheNode) =>
+                assert s'.sequence_attestation_duties_to_be_served == s.sequence_attestation_duties_to_be_served;
+        }
+        assert s'.sequence_attestation_duties_to_be_served == s.sequence_attestation_duties_to_be_served;
+
+    }
+
+    // TODO: Simplify
+    lemma lem_inv_data_of_att_share_is_decided_value_att_consensus_decided_helper_1(
+        s: DVState,
+        event: DV.Event,
+        s': DVState,
+        hn: BLSPubkey,
+        att_share: AttestationShare
+    )
+    requires NextEventPreCond(s, event)
+    requires NextEvent(s, event, s')  
+    requires event.HonestNodeTakingStep?
+    requires event.event.AttConsensusDecided?
+    requires inv_data_of_att_share_is_decided_value(s)
+    requires inv_decided_value_of_consensus_instance_of_slot_k_is_for_slot_k(s)
+    requires inv_attestation_shares_to_broadcast_is_a_subset_of_all_messages_sent(s)  
+    requires inv_quorum_constraints(s)
+    requires inv_unchanged_honesty(s)
+    requires same_honest_nodes_in_dv_and_ci(s)
+    requires inv_only_dv_construct_signed_attestation_signature(s)
+    requires inv_decided_value_of_consensus_instance_is_decided_by_quorum(s)    
+    requires inv_sent_validity_predicate_is_based_on_rcvd_att_duty_and_slashing_db(s)
+    requires inv_sent_validity_predicate_is_based_on_rcvd_att_duty_and_slashing_db_for_dv(s)          
+    requires |s.all_nodes| > 0    
+    requires is_correct_att_share(s, hn, att_share)
+    requires att_share in s.att_network.allMessagesSent
+    ensures && s'.consensus_on_attestation_data[att_share.data.slot].decided_value.isPresent()                                     
+            && s'.consensus_on_attestation_data[att_share.data.slot].decided_value.safe_get() == att_share.data
+    {
+        match event 
+        {
+            case HonestNodeTakingStep(node, nodeEvent, nodeOutputs) =>
+                var s_node := s.honest_nodes_states[node];
+                var s'_node := s'.honest_nodes_states[node];
+                match nodeEvent
+                {
+                    case AttConsensusDecided(id: Slot, decided_attestation_data) => 
+                        assert att_share in s.att_network.allMessagesSent;
+                        assert inv_data_of_att_share_is_decided_value(s);
+                        assert inv_data_of_att_share_is_decided_value_body(s, att_share);
+                        assert s.consensus_on_attestation_data[att_share.data.slot].decided_value.isPresent();
+                        assert s.consensus_on_attestation_data[att_share.data.slot].decided_value.safe_get() == att_share.data;   
+
+                        var s_w_honest_node_states_updated := lem_inv_sent_validity_predicate_is_based_on_rcvd_att_duty_and_slashing_db_get_s_w_honest_node_states_updated(s, node, nodeEvent);           
+                        var cid := att_share.data.slot;
+
+                        assert s_w_honest_node_states_updated.consensus_on_attestation_data == s.consensus_on_attestation_data;
+
+                        var output := 
+                            if nodeEvent.AttConsensusDecided? && nodeEvent.id == cid then 
+                                Some(Decided(node, nodeEvent.decided_attestation_data))
+                            else
+                                None
+                            ;
+
+                        var validityPredicates := 
+                            map n |
+                                    && n in s_w_honest_node_states_updated.honest_nodes_states.Keys 
+                                    && cid in s_w_honest_node_states_updated.honest_nodes_states[n].attestation_consensus_engine_state.active_attestation_consensus_instances.Keys
+                                ::
+                                    s_w_honest_node_states_updated.honest_nodes_states[n].attestation_consensus_engine_state.active_attestation_consensus_instances[cid].validityPredicate
+                            ;
+
+                        var s_consensus := s_w_honest_node_states_updated.consensus_on_attestation_data[cid];
+                        var s'_consensus := s'.consensus_on_attestation_data[cid];                
+
+                        assert
+                            ConsensusSpec.Next(
+                                s_consensus,
+                                validityPredicates,
+                                s'_consensus,
+                                output
+                            );      
+
+                        lem_consensus_next_under_safety(
+                            s_consensus,
+                            validityPredicates,
+                            s'_consensus,
+                            output                                
+                        );                        
+                            
+                        assert s'.consensus_on_attestation_data[att_share.data.slot].decided_value.isPresent();
+                        assert s.consensus_on_attestation_data[att_share.data.slot].decided_value.safe_get() == s'.consensus_on_attestation_data[att_share.data.slot].decided_value.safe_get();
+                            assert s'.consensus_on_attestation_data[att_share.data.slot].decided_value.safe_get() == att_share.data;
+                }
+        }
+    }
+
+    // // Ver time: 1m 35s
+    // IMPORTANT: Seem to be an error of Dafny with the second match expression
+    // lemma lem_inv_data_of_att_share_is_decided_value(
+    //     s: DVState,
+    //     event: DV.Event,
+    //     s': DVState
+    // )
+    // requires NextEventPreCond(s, event)
+    // requires NextEvent(s, event, s')  
+    // requires inv_quorum_constraints(s)
+    // requires inv_unchanged_honesty(s)
+    // requires same_honest_nodes_in_dv_and_ci(s)
+    // requires inv_only_dv_construct_signed_attestation_signature(s)
+    // requires inv_data_of_att_share_is_decided_value(s)
+    // requires inv_decided_value_of_consensus_instance_of_slot_k_is_for_slot_k(s)
+    // requires inv_attestation_shares_to_broadcast_is_a_subset_of_all_messages_sent(s)      
+    // requires inv_decided_value_of_consensus_instance_is_decided_by_quorum(s)    
+    // requires inv_sent_validity_predicate_is_based_on_rcvd_att_duty_and_slashing_db(s)    
+    // requires inv_sent_validity_predicate_is_based_on_rcvd_att_duty_and_slashing_db_for_dv(s)          
+    // requires |s.all_nodes| > 0
+    // // ensures inv_data_of_att_share_is_decided_value(s')   
+    // {
+    //     match event 
+    //     {
+    //         case HonestNodeTakingStep(node, nodeEvent, nodeOutputs) =>
+    //             var s_node := s.honest_nodes_states[node];
+    //             var s'_node := s'.honest_nodes_states[node];
+    //             if nodeEvent.AttConsensusDecided? 
+    //             {
+    //                 // lem_inv_data_of_att_share_is_decided_value_att_consensus_decided(s, event, s');
+    //             }
+    //             else 
+    //             {
+    //                 match nodeEvent
+    //                 {
+    //                     // case ServeAttstationDuty(attestation_duty) => 
+    //                     //     var messagesToBeSent := f_serve_attestation_duty(s_node, attestation_duty).outputs.att_shares_sent;
+    //                     //     assert s'.att_network.allMessagesSent == s.att_network.allMessagesSent + 
+    //                     //         getMessagesFromMessagesWithRecipient(messagesToBeSent);
+    //                     //     lem_f_serve_attestation_duty_constants(s_node, attestation_duty, s'_node);
+    //                     //     assert messagesToBeSent == {};
+    //                     //     lem_inv_data_of_att_share_is_decided_value_helper2(s'.att_network.allMessagesSent, s.att_network.allMessagesSent, messagesToBeSent);
+    //                     //     assert s'.att_network.allMessagesSent == s.att_network.allMessagesSent;
+                            
+                                                                    
+    //                     // case ReceivedAttestationShare(attestation_share) => 
+    //                     //     var messagesToBeSent := f_listen_for_attestation_shares(s_node, attestation_share).outputs.att_shares_sent;
+    //                     //     assert messagesToBeSent == {};                        
+    //                     //     assert s'.att_network.allMessagesSent == 
+    //                     //                 s.att_network.allMessagesSent + getMessagesFromMessagesWithRecipient(messagesToBeSent);
+    //                     //     assert s'.att_network.allMessagesSent == 
+    //                     //                 s.att_network.allMessagesSent + getMessagesFromMessagesWithRecipient({});                                              
+
+    //                     // case ImportedNewBlock(block) => 
+    //                     //     var s_node := f_add_block_to_bn(s_node, nodeEvent.block);
+    //                     //     var messagesToBeSent := f_listen_for_new_imported_blocks(s_node, block).outputs.att_shares_sent;
+    //                     //     assert s'.att_network.allMessagesSent == 
+    //                     //                 s.att_network.allMessagesSent + getMessagesFromMessagesWithRecipient(messagesToBeSent);
+    //                     //     lem_f_listen_for_new_imported_blocksd_unchanged_dvc_vars(s_node, block, s'_node);
+    //                     //     assert messagesToBeSent == {};
+    //                     //     lem_inv_data_of_att_share_is_decided_value_helper2(s'.att_network.allMessagesSent, s.att_network.allMessagesSent, messagesToBeSent);
+    //                     //     assert s'.att_network.allMessagesSent == s.att_network.allMessagesSent;                 
+                    
+    //                     // case ResendAttestationShares => 
+    //                     //     var messagesToBeSent := f_resend_attestation_share(s_node).outputs.att_shares_sent;     
+
+    //                     //     assert s'.att_network.allMessagesSent == 
+    //                     //                 s.att_network.allMessagesSent + getMessagesFromMessagesWithRecipient(messagesToBeSent);  
+
+    //                     //     forall m | m in getMessagesFromMessagesWithRecipient(messagesToBeSent)  
+    //                     //     ensures m in s.att_network.allMessagesSent
+    //                     //     {
+    //                     //         assert m in s_node.attestation_shares_to_broadcast.Values;
+    //                     //         assert m in s.att_network.allMessagesSent;
+    //                     //     }        
+
+    //                     //     assert s'.att_network.allMessagesSent == s.att_network.allMessagesSent;
+
+    //                     // case NoEvent => 
+    //                     //     assert s'.att_network == s.att_network;
+    //                 }
+    //                 // lem_inv_data_of_att_share_is_decided_value_helper(s, event, s');
+    //             }
+
+
+    //         case AdeversaryTakingStep(node, new_attestation_share_sent, messagesReceivedByTheNode) =>
+    //         //     lem_inv_data_of_att_share_is_decided_value_att_adversary(s, event, s');
+    //     }        
+    // }
+
+    lemma lem_inv_data_of_att_share_is_decided_value(
+        s: DVState,
+        event: DV.Event,
+        s': DVState
+    )
+    requires NextEventPreCond(s, event)
+    requires NextEvent(s, event, s')  
+    requires inv_quorum_constraints(s)
+    requires inv_unchanged_honesty(s)
+    requires same_honest_nodes_in_dv_and_ci(s)
+    requires inv_only_dv_construct_signed_attestation_signature(s)
+    requires inv_data_of_att_share_is_decided_value(s)
+    requires inv_decided_value_of_consensus_instance_of_slot_k_is_for_slot_k(s)
+    requires inv_attestation_shares_to_broadcast_is_a_subset_of_all_messages_sent(s)      
+    requires inv_decided_value_of_consensus_instance_is_decided_by_quorum(s)    
+    requires inv_sent_validity_predicate_is_based_on_rcvd_att_duty_and_slashing_db(s)    
+    requires inv_sent_validity_predicate_is_based_on_rcvd_att_duty_and_slashing_db_for_dv(s)          
+    requires |s.all_nodes| > 0
+    ensures inv_data_of_att_share_is_decided_value(s')   
+    {
+        match event 
+        {
+            case HonestNodeTakingStep(node, nodeEvent, nodeOutputs) =>
+                var s_node := s.honest_nodes_states[node];
+                var s'_node := s'.honest_nodes_states[node];
+                if nodeEvent.AttConsensusDecided? 
+                {
+                    lem_inv_data_of_att_share_is_decided_value_att_consensus_decided(s, event, s');
+                }
+                else 
+                {
+                    match nodeEvent
+                    {
+                        case ServeAttstationDuty(attestation_duty) => 
+                            var messagesToBeSent := f_serve_attestation_duty(s_node, attestation_duty).outputs.att_shares_sent;
+                            assert s'.att_network.allMessagesSent == 
+                                        s.att_network.allMessagesSent + getMessagesFromMessagesWithRecipient(messagesToBeSent);
+                            lem_f_serve_attestation_duty_constants(s_node, attestation_duty, s'_node);
+                            assert messagesToBeSent == {};
+                            lem_inv_data_of_att_share_is_decided_value_helper2(s'.att_network.allMessagesSent, s.att_network.allMessagesSent, messagesToBeSent);
+                            assert s'.att_network.allMessagesSent == s.att_network.allMessagesSent;
+                            
+                                                                    
+                        case ReceivedAttestationShare(attestation_share) => 
+                            var messagesToBeSent := f_listen_for_attestation_shares(s_node, attestation_share).outputs.att_shares_sent;
+                            assert messagesToBeSent == {};                        
+                            assert s'.att_network.allMessagesSent == 
+                                        s.att_network.allMessagesSent + getMessagesFromMessagesWithRecipient(messagesToBeSent);
+                            assert s'.att_network.allMessagesSent == 
+                                        s.att_network.allMessagesSent + getMessagesFromMessagesWithRecipient({});                                              
+
+                        case ImportedNewBlock(block) => 
+                            var s_node := f_add_block_to_bn(s_node, nodeEvent.block);
+                            var messagesToBeSent := f_listen_for_new_imported_blocks(s_node, block).outputs.att_shares_sent;
+                            assert s'.att_network.allMessagesSent == 
+                                        s.att_network.allMessagesSent + getMessagesFromMessagesWithRecipient(messagesToBeSent);
+                            lem_f_listen_for_new_imported_blocksd_unchanged_dvc_vars(s_node, block, s'_node);
+                            assert messagesToBeSent == {};
+                            lem_inv_data_of_att_share_is_decided_value_helper2(s'.att_network.allMessagesSent, s.att_network.allMessagesSent, messagesToBeSent);
+                            assert s'.att_network.allMessagesSent == s.att_network.allMessagesSent;                 
+                    
+                        case ResendAttestationShares => 
+                            var messagesToBeSent := f_resend_attestation_share(s_node).outputs.att_shares_sent;     
+
+                            assert s'.att_network.allMessagesSent == 
+                                        s.att_network.allMessagesSent + getMessagesFromMessagesWithRecipient(messagesToBeSent);  
+
+                            forall m | m in getMessagesFromMessagesWithRecipient(messagesToBeSent)  
+                            ensures m in s.att_network.allMessagesSent
+                            {
+                                assert m in s_node.attestation_shares_to_broadcast.Values;
+                                assert m in s.att_network.allMessagesSent;
+                            }        
+
+                            assert s'.att_network.allMessagesSent == s.att_network.allMessagesSent;
+
+                        case NoEvent => 
+                            assert s'.att_network == s.att_network;
+                    }
+                    lem_inv_data_of_att_share_is_decided_value_helper(s, event, s');
+                }
+
+            case AdeversaryTakingStep(node, new_attestation_share_sent, messagesReceivedByTheNode) =>
+                lem_inv_data_of_att_share_is_decided_value_att_adversary(s, event, s');
+        }        
+    }
+}
